Improving the verification technique. Channel invariants are now inhaled/exhaled in the same way as network invariants at action entries. This avoids repeating information and also makes the verification technique more "uniform". There seems to be no real problems with doing this.

src/fi/abo/it/actortool/boogie/Translator.scala
@@ -280,8 +280,6 @@ class Translator(val fixedBaseLength: Int, val ftMode: Boolean, implicit val bvM
       (buffer.toMap,decls.toList)
     }
     
-    val bChInvs = for (chi <- chInvariants) yield ((chi,transExpr(chi.expr)(networkRenamings)))
-    
     val (sourceMap,targetMap) = {
       val source = scala.collection.mutable.HashMap.empty[PortRef,List[String]]
       val target = scala.collection.mutable.HashMap.empty[PortRef,String]
@@ -292,12 +290,12 @@ class Translator(val fixedBaseLength: Int, val ftMode: Boolean, implicit val bvM
       }
       (source.toMap,target.toMap)
     }
-    decls ++= translateNetworkInit(nwInvariants, bChInvs, networkRenamings, 
+    decls ++= translateNetworkInit(nwInvariants, chInvariants, networkRenamings, 
         sourceMap, targetMap, entities, connections, network.id+Sep)
 
     for (a <- actions) {
       decls ++= translateNetworkAction(
-          a,nwInvariants,bChInvs,networkRenamings,sourceMap,targetMap,
+          a,nwInvariants,chInvariants,networkRenamings,sourceMap,targetMap,
           entities,connections,subactorVarDecls,network.id+Sep)
     }
 
@@ -306,7 +304,7 @@ class Translator(val fixedBaseLength: Int, val ftMode: Boolean, implicit val bvM
   
   def translateNetworkInit(
        nwInvs: List[ActorInvariant],
-       chInvs: List[(ChannelInvariant,Boogie.Expr)],
+       chInvs: List[ChannelInvariant],
        networkRenamings: Map[String,String], // Channels and entities
        sourceMap: Map[PortRef,List[String]],
        targetMap: Map[PortRef,String],
@@ -371,7 +369,7 @@ class Translator(val fixedBaseLength: Int, val ftMode: Boolean, implicit val bvM
   def translateNetworkAction(
        nwa: Action, 
        nwInvs: List[ActorInvariant],
-       chInvs: List[(ChannelInvariant,Boogie.Expr)],
+       chInvs: List[ChannelInvariant],
        networkRenamings: Map[String,String], // Channels and entities
        sourceMap: Map[PortRef,List[String]],
        targetMap: Map[PortRef,String],
@@ -409,11 +407,8 @@ class Translator(val fixedBaseLength: Int, val ftMode: Boolean, implicit val bvM
         case PortRef(None,p) =>
           limitAssumesBuffer += bAssume(bCredInit(networkRenamings(c.id)) ==@ bInt(nwa.portInputCount(p))*bBaseL)
           limitLoopCondBuffer += bTotal(networkRenamings(c.id)) < bCredInit(networkRenamings(c.id))
-        //case PortRef(_,_) => 
-        //  cInitAssumesBuffer += bAssume(bCredInit(networkRenamings(c.id)) ==@ bInt(0))
         case _ =>
       }
-      assumesBuffer += bAssume(bRead(networkRenamings(c.id)) ==@ bInt(0))
       assumesBuffer += bAssume(bCredit(networkRenamings(c.id)) ==@ bInt(0))
     }
     
@@ -441,11 +436,7 @@ class Translator(val fixedBaseLength: Int, val ftMode: Boolean, implicit val bvM
       val outChan = Id(targetMap(PortRef(None,portId))); outChan.typ = ChanType(decl.typ)
       val acc = IndexAccessor(outChan,IntLiteral(index))
       Resolver.resolveExpr(acc)
-      replacements = replacements + (Id(decl.id) -> acc)
-      /*val newName = "ActionPH"+Sep+placeHolder.id
-      procVars += bLocal(newName,type2BType(placeHolder.typ))
-      actionRenamings += ((placeHolder.id,newName))*/
-      
+      replacements = replacements + (Id(decl.id) -> acc)      
     }
 
     val outputs = (for (opat <- nwa.outputPattern) yield {
@@ -460,18 +451,11 @@ class Translator(val fixedBaseLength: Int, val ftMode: Boolean, implicit val bvM
         
         val stmts =
           if (e.isInstanceOf[Id] && (nwa.placeHolderVars exists {case (d,p,i) => d.id == e.asInstanceOf[Id].id  })) {
-            // If this is an action variable it will be used as a placeholder
-//            val v = transExpr(e)(renamings)
-//            List(Boogie.Assign(v,transExpr(acc)(renamings)))
             Nil
           }
           else {
-            /*val name = prefix+opat.portId+Sep+i
-            procVars += bLocal(name,type2BType(e.typ))
-            val v = VarExpr(name)*/
-            List(
-                /*Boogie.Assign(v,transExpr(acc)(renamings)),*/
-                bAssert(transExpr(acc)(renamings) ==@ transExpr(renamedExp)(renamings),e.pos,"Network output might not conform to the specified action output"))    
+            List(bAssert(transExpr(acc)(renamings) ==@ transExpr(renamedExp)(renamings),
+                e.pos,"Network output might not conform to the specified action output"))    
           }
         i = i+1
         stmts
@@ -489,6 +473,7 @@ class Translator(val fixedBaseLength: Int, val ftMode: Boolean, implicit val bvM
     val nwPost = for (q <- nwa.ensures) yield 
       (q.pos,transExpr(IdReplacer.visitExpr(q)(replacements))(renamings))
 
+      
     // Network action entry
     val entryStmt = 
       procVars.toList :::
@@ -498,12 +483,17 @@ class Translator(val fixedBaseLength: Int, val ftMode: Boolean, implicit val bvM
       //stepAssumes :::
       //List(bAssume(VarExpr("C#init") ==@ VarExpr("C"))) :::
       (for (nwi <- nwInvs) yield Inhalator.visit(nwi, networkRenamings)).flatten :::
+      (for (chi <- chInvs) yield Inhalator.visit(chi, networkRenamings)).flatten :::
       nwPre:::
-      (for ((chi,bChi) <- chInvs) yield {
-        val baseMsg = "Channel invariant might not hold on action entry"
-        val msg = baseMsg + " (" + GeneratedInvariantCount.next + ")"
-        if (!chi.assertion.free) bAssert(bChi,chi.pos,msg) else bAssume(bChi)
-      })
+      (for (chi <- chInvs) yield {
+        if (!chi.assertion.free) {
+          val baseMsg = "Channel invariant might not hold on action entry"
+          val msg = baseMsg + " (" + GeneratedInvariantCount.next + ")"
+          Exhalator.visit(chi,msg,renamings)
+        }
+        else Nil
+        //if (!chi.assertion.free) bAssert(bChi,chi.pos,msg) else bAssume(bChi)
+      }).flatten
     val initProc = Boogie.Proc(Uniquifier.get(prefix+nwa.fullName+"#entry"),Nil,Nil,Modifies,Nil,entryStmt)
     
     // Sub-actor executions
@@ -563,7 +553,7 @@ class Translator(val fixedBaseLength: Int, val ftMode: Boolean, implicit val bvM
     val exitStmt =
       procVars.toList:::
       cInitAssumes:::
-      (for ((_,chi) <- chInvs) yield bAssume(chi)):::
+      (for (chi <- chInvs) yield Inhalator.visit(chi,"",renamings)).flatten:::
       limitNegAssumes:::
       firingNegAssumes:::
       outputs:::
@@ -587,6 +577,10 @@ class Translator(val fixedBaseLength: Int, val ftMode: Boolean, implicit val bvM
           case _ => Nil
         }
       }).flatten:::
+      //
+      (for (chi <- chInvs) yield 
+        Exhalator.visit(chi,"The network might not preserve the channel invariant",networkRenamings)).flatten :::
+      //
       (for (nwi <- nwInvs) yield 
         Exhalator.visit(nwi,"The network might not preserve the network invariant",networkRenamings)).flatten :::
       (for (c <- connections) yield {
@@ -612,7 +606,7 @@ class Translator(val fixedBaseLength: Int, val ftMode: Boolean, implicit val bvM
       action: Action, 
       networkRenamings: Map[String,String], // Channels and entities
       cInits: List[Boogie.Assume],
-      chInvs: List[(ChannelInvariant,Boogie.Expr)],
+      chInvs: List[ChannelInvariant],
       sourceMap: Map[PortRef,List[String]], 
       targetMap: Map[PortRef,String],
       priorityGuard: List[Boogie.Expr]): (List[Boogie.Stmt],List[Boogie.LocalVar],Boogie.Expr,Boogie.Expr) = {
@@ -636,7 +630,7 @@ class Translator(val fixedBaseLength: Int, val ftMode: Boolean, implicit val bvM
     }
     
     asgn ++= cInits // Assumptions about initial state of channels
-    asgn ++= (for ((_,chi) <- chInvs) yield bAssume(chi))  // Assume channel invariants
+    asgn ++= (for (chi <- chInvs) yield Inhalator.visit(chi, "", networkRenamings)).flatten  // Assume channel invariants
     
     
     val actorRenamings = networkRenamings ++ actorParamRenames //++ actorVarRenames
@@ -778,13 +772,18 @@ class Translator(val fixedBaseLength: Int, val ftMode: Boolean, implicit val bvM
       asgn += Boogie.Assign(bSqnAct(instanceBName),bSqnAct(instanceBName) plus bInt(1))
     }
     
-    asgn ++= (for ((chi,bChi) <- chInvs) yield {
-      val baseMsg = 
-        "Action at " + action.pos + " ('" + action.fullName + "') for actor instance '" + 
-        instance.id + "' might not preserve the channel invariant"
-      val msg = baseMsg + " (" + GeneratedInvariantCount.next + ")"
-      if (!chi.assertion.free) bAssert(bChi,chi.pos,msg) else bAssume(bChi)
-    })
+    asgn ++= (for (chi <- chInvs) yield {
+      if (!chi.assertion.free) {
+        val baseMsg = 
+          "Action at " + action.pos + " ('" + action.fullName + "') for actor instance '" + 
+          instance.id + "' might not preserve the channel invariant"
+        val msg = baseMsg + " (" + GeneratedInvariantCount.next + ")"
+        Exhalator.visit(chi, msg, networkRenamings)
+      }
+      else {
+        Nil
+      }
+    }).flatten
             
     (asgn.toList, newVars.toList, firingRuleWithPrio, firingRuleWithoutPrio)
   }
@@ -797,10 +796,19 @@ class Translator(val fixedBaseLength: Int, val ftMode: Boolean, implicit val bvM
   abstract class Halator(val inhale: Boolean) {
     import Helper._
     
+    def visit(inv: ChannelInvariant, renamings: Map[String,String]): List[Boogie.Stmt] = 
+      visit(inv, "Invariant might not hold", renamings)
+    
     def visit(inv: ActorInvariant, renamings: Map[String,String]): List[Boogie.Stmt] = 
       visit(inv, "Invariant might not hold", renamings)
     
     def visit(inv: ActorInvariant, msg: String, renamings: Map[String,String]): List[Boogie.Stmt] = {
+      val buffer = new ListBuffer[Boogie.Stmt]
+      visit(inv.expr, inv.assertion.free)(buffer,msg,renamings);
+      buffer.toList
+    }
+    
+    def visit(inv: ChannelInvariant, msg: String, renamings: Map[String,String]): List[Boogie.Stmt] = {
       val buffer = new ListBuffer[Boogie.Stmt]
       visit(inv.expr, inv.assertion.free)(buffer,msg,renamings);
       buffer.toList
