ft_tests/Timeout.bpl
@@ -134,19 +134,12 @@ procedure Net#anon$3#entry#7()
   assume SqnAct[Net#sec] == 0;
   assume SqnAct[Net#adj] == 0;
   assume L[Net#a] == (1 * Base#L);
-  assume R[Net#a] == 0;
   assume C[Net#a] == 0;
-  assume R[Net#b] == 0;
   assume C[Net#b] == 0;
-  assume R[Net#c] == 0;
   assume C[Net#c] == 0;
-  assume R[Net#d] == 0;
   assume C[Net#d] == 0;
-  assume R[Net#e] == 0;
   assume C[Net#e] == 0;
-  assume R[Net#f] == 0;
   assume C[Net#f] == 0;
-  assume R[Net#g] == 0;
   assume C[Net#g] == 0;
   C[Net#f] := C[Net#f] + 1;
   assume R[Net#e] == M[Net#f][R[Net#f]];
@@ -167,55 +160,161 @@ procedure Net#anon$3#entry#7()
   assume 0 <= R[Net#g];
   assume 0 <= C[Net#g];
   assume R[Net#g] == 0;
-  assert {:msg "  Channel invariant might not hold on action entry (#16)"} R[Net#a] == (R[Net#b] + C[Net#b]);
-  assert {:msg "  Channel invariant might not hold on action entry (#17)"} R[Net#a] == (R[Net#c] + C[Net#c]);
-  assert {:msg "  Channel invariant might not hold on action entry (#18)"} R[Net#b] == (R[Net#d] + C[Net#d]);
-  assert {:msg "  Channel invariant might not hold on action entry (#19)"} R[Net#c] == (R[Net#e] + C[Net#e]);
-  assert {:msg "  Channel invariant might not hold on action entry (#20)"} (forall idx$: int :: 
+  assume R[Net#a] == (R[Net#b] + C[Net#b]);
+  assert {:msg "  Invariant might not hold"} R[Net#a] == (R[Net#b] + C[Net#b]);
+  assume R[Net#a] == (R[Net#c] + C[Net#c]);
+  assert {:msg "  Invariant might not hold"} R[Net#a] == (R[Net#c] + C[Net#c]);
+  assume R[Net#b] == (R[Net#d] + C[Net#d]);
+  assert {:msg "  Invariant might not hold"} R[Net#b] == (R[Net#d] + C[Net#d]);
+  assume R[Net#c] == (R[Net#e] + C[Net#e]);
+  assert {:msg "  Invariant might not hold"} R[Net#c] == (R[Net#e] + C[Net#e]);
+  assume (forall idx$: int :: 
     (0 <= idx$) && (idx$ < (R[Net#b] + C[Net#b])) ==> (M[Net#b][idx$] == M[Net#a][idx$])
   );
-  assert {:msg "  Channel invariant might not hold on action entry (#21)"} (forall idx$: int :: 
+  assert {:msg "  Invariant might not hold"} (forall idx$: int :: 
+    (0 <= idx$) && (idx$ < (R[Net#b] + C[Net#b])) ==> (M[Net#b][idx$] == M[Net#a][idx$])
+  );
+  assume (forall idx$: int :: 
     (0 <= idx$) && (idx$ < (R[Net#c] + C[Net#c])) ==> (M[Net#c][idx$] == M[Net#a][idx$])
   );
-  assert {:msg "  Channel invariant might not hold on action entry (#22)"} (forall idx$: int :: 
+  assert {:msg "  Invariant might not hold"} (forall idx$: int :: 
+    (0 <= idx$) && (idx$ < (R[Net#c] + C[Net#c])) ==> (M[Net#c][idx$] == M[Net#a][idx$])
+  );
+  assume (forall idx$: int :: 
     (0 <= idx$) && (idx$ < (R[Net#d] + C[Net#d])) ==> (M[Net#d][idx$] == M[Net#b][idx$])
   );
-  assert {:msg "  Channel invariant might not hold on action entry (#23)"} (forall idx$: int :: 
+  assert {:msg "  Invariant might not hold"} (forall idx$: int :: 
+    (0 <= idx$) && (idx$ < (R[Net#d] + C[Net#d])) ==> (M[Net#d][idx$] == M[Net#b][idx$])
+  );
+  assume (forall idx$: int :: 
     (0 <= idx$) && (idx$ < (R[Net#e] + C[Net#e])) ==> (M[Net#e][idx$] == M[Net#c][idx$])
   );
-  assert {:msg "  Channel invariant might not hold on action entry (#24)"} (forall idx$: int :: 
+  assert {:msg "  Invariant might not hold"} (forall idx$: int :: 
+    (0 <= idx$) && (idx$ < (R[Net#e] + C[Net#e])) ==> (M[Net#e][idx$] == M[Net#c][idx$])
+  );
+  assume (forall idx$: int :: 
     (0 <= idx$) && (idx$ < (R[Net#a] + C[Net#a])) ==> (SqnCh[Net#a][idx$] == idx$)
   );
-  assert {:msg "  40.3: Channel invariant might not hold on action entry (#25)"} SqnAct[Net#spl] == R[Net#a];
-  assert {:msg "  41.3: Channel invariant might not hold on action entry (#26)"} SqnAct[Net#pri] == R[Net#b];
-  assert {:msg "  42.3: Channel invariant might not hold on action entry (#27)"} SqnAct[Net#sec] == R[Net#c];
-  assert {:msg "  43.3: Channel invariant might not hold on action entry (#28)"} SqnAct[Net#adj] == R[Net#e];
-  assert {:msg "  45.3: Channel invariant might not hold on action entry (#29)"} (forall i: int :: 
+  assert {:msg "  Invariant might not hold"} (forall idx$: int :: 
+    (0 <= idx$) && (idx$ < (R[Net#a] + C[Net#a])) ==> (SqnCh[Net#a][idx$] == idx$)
+  );
+  assume SqnAct[Net#spl] == R[Net#a];
+  assert {:msg "  40.15: Invariant might not hold"} SqnAct[Net#spl] == R[Net#a];
+  assume SqnAct[Net#pri] == R[Net#b];
+  assert {:msg "  41.15: Invariant might not hold"} SqnAct[Net#pri] == R[Net#b];
+  assume SqnAct[Net#sec] == R[Net#c];
+  assert {:msg "  42.15: Invariant might not hold"} SqnAct[Net#sec] == R[Net#c];
+  assume SqnAct[Net#adj] == R[Net#e];
+  assert {:msg "  43.15: Invariant might not hold"} SqnAct[Net#adj] == R[Net#e];
+  assume (forall i: int :: 
     (0 <= i) && (i < (R[Net#a] + C[Net#a])) ==> (SqnCh[Net#a][i] == i)
   );
-  assert {:msg "  46.3: Channel invariant might not hold on action entry (#30)"} (forall i: int :: 
+  assert {:msg "  45.16: Invariant might not hold"} (forall i: int :: 
+    (0 <= i) && (i < (R[Net#a] + C[Net#a])) ==> (SqnCh[Net#a][i] == i)
+  );
+  assume (forall i: int :: 
     (0 <= i) && (i < (R[Net#b] + C[Net#b])) ==> (SqnCh[Net#b][i] == i)
   );
-  assert {:msg "  47.3: Channel invariant might not hold on action entry (#31)"} (forall i: int :: 
+  assert {:msg "  46.16: Invariant might not hold"} (forall i: int :: 
+    (0 <= i) && (i < (R[Net#b] + C[Net#b])) ==> (SqnCh[Net#b][i] == i)
+  );
+  assume (forall i: int :: 
     (0 <= i) && (i < (R[Net#c] + C[Net#c])) ==> (SqnCh[Net#c][i] == i)
   );
-  assert {:msg "  48.3: Channel invariant might not hold on action entry (#32)"} (forall i: int :: 
+  assert {:msg "  47.16: Invariant might not hold"} (forall i: int :: 
+    (0 <= i) && (i < (R[Net#c] + C[Net#c])) ==> (SqnCh[Net#c][i] == i)
+  );
+  assume (forall i: int :: 
     (0 <= i) && (i < (R[Net#d] + C[Net#d])) ==> (SqnCh[Net#d][i] == i)
   );
-  assert {:msg "  49.3: Channel invariant might not hold on action entry (#33)"} (forall i: int :: 
+  assert {:msg "  48.16: Invariant might not hold"} (forall i: int :: 
+    (0 <= i) && (i < (R[Net#d] + C[Net#d])) ==> (SqnCh[Net#d][i] == i)
+  );
+  assume (forall i: int :: 
     (0 <= i) && (i < (R[Net#e] + C[Net#e])) ==> (SqnCh[Net#e][i] == i)
   );
-  assert {:msg "  50.3: Channel invariant might not hold on action entry (#34)"} (forall i: int :: 
+  assert {:msg "  49.16: Invariant might not hold"} (forall i: int :: 
+    (0 <= i) && (i < (R[Net#e] + C[Net#e])) ==> (SqnCh[Net#e][i] == i)
+  );
+  assume (forall i: int :: 
     (0 <= i) && (i < (R[Net#g] + C[Net#g])) ==> (SqnCh[Net#g][i] == i)
   );
-  assert {:msg "  52.3: Channel invariant might not hold on action entry (#35)"} C[Net#f] == 1;
-  assert {:msg "  53.3: Channel invariant might not hold on action entry (#36)"} C[Net#g] == R[Net#e];
-  assert {:msg "  54.3: Channel invariant might not hold on action entry (#37)"} R[Net#e] == M[Net#f][R[Net#f]];
-  assert {:msg "  55.3: Channel invariant might not hold on action entry (#38)"} (forall i: int :: 
+  assert {:msg "  50.16: Invariant might not hold"} (forall i: int :: 
     (0 <= i) && (i < (R[Net#g] + C[Net#g])) ==> (SqnCh[Net#g][i] == i)
   );
-  assert {:msg "  59.3: Channel invariant might not hold on action entry (#39)"} (0 < R[Net#d]) && (0 < R[Net#e]) ==> (M[Net#d][R[Net#d] - 1] <= M[Net#e][R[Net#e] - 1]);
-  assert {:msg "  60.3: Channel invariant might not hold on action entry (#40)"} (forall i: int :: 
+  assume C[Net#f] == 1;
+  assert {:msg "  52.15: Invariant might not hold"} C[Net#f] == 1;
+  assume (R[Net#g] + C[Net#g]) == R[Net#e];
+  assert {:msg "  53.15: Invariant might not hold"} (R[Net#g] + C[Net#g]) == R[Net#e];
+  assume R[Net#e] == M[Net#f][R[Net#f]];
+  assert {:msg "  54.15: Invariant might not hold"} R[Net#e] == M[Net#f][R[Net#f]];
+  assume (forall i: int :: 
+    (0 <= i) && (i < (R[Net#g] + C[Net#g])) ==> (SqnCh[Net#g][i] == i)
+  );
+  assert {:msg "  55.16: Invariant might not hold"} (forall i: int :: 
+    (0 <= i) && (i < (R[Net#g] + C[Net#g])) ==> (SqnCh[Net#g][i] == i)
+  );
+  if ((0 < R[Net#d]) && (0 < R[Net#e])) {
+    assume M[Net#d][R[Net#d] - 1] <= M[Net#e][R[Net#e] - 1];
+    assert {:msg "  57.42: Invariant might not hold"} M[Net#d][R[Net#d] - 1] <= M[Net#e][R[Net#e] - 1];
+  }
+  assume (forall i: int :: 
+    (0 <= i) && (i < R[Net#e]) ==> (M[Net#g][i] == M[Net#e][i])
+  );
+  assert {:msg "  58.16: Invariant might not hold"} (forall i: int :: 
+    (0 <= i) && (i < R[Net#e]) ==> (M[Net#g][i] == M[Net#e][i])
+  );
+  assert {:msg "  Channel invariant might not hold on action entry (#0)"} R[Net#a] == (R[Net#b] + C[Net#b]);
+  assert {:msg "  Channel invariant might not hold on action entry (#1)"} R[Net#a] == (R[Net#c] + C[Net#c]);
+  assert {:msg "  Channel invariant might not hold on action entry (#2)"} R[Net#b] == (R[Net#d] + C[Net#d]);
+  assert {:msg "  Channel invariant might not hold on action entry (#3)"} R[Net#c] == (R[Net#e] + C[Net#e]);
+  assert {:msg "  Channel invariant might not hold on action entry (#4)"} (forall idx$: int :: 
+    (0 <= idx$) && (idx$ < (R[Net#b] + C[Net#b])) ==> (M[Net#b][idx$] == M[Net#a][idx$])
+  );
+  assert {:msg "  Channel invariant might not hold on action entry (#5)"} (forall idx$: int :: 
+    (0 <= idx$) && (idx$ < (R[Net#c] + C[Net#c])) ==> (M[Net#c][idx$] == M[Net#a][idx$])
+  );
+  assert {:msg "  Channel invariant might not hold on action entry (#6)"} (forall idx$: int :: 
+    (0 <= idx$) && (idx$ < (R[Net#d] + C[Net#d])) ==> (M[Net#d][idx$] == M[Net#b][idx$])
+  );
+  assert {:msg "  Channel invariant might not hold on action entry (#7)"} (forall idx$: int :: 
+    (0 <= idx$) && (idx$ < (R[Net#e] + C[Net#e])) ==> (M[Net#e][idx$] == M[Net#c][idx$])
+  );
+  assert {:msg "  Channel invariant might not hold on action entry (#8)"} (forall idx$: int :: 
+    (0 <= idx$) && (idx$ < (R[Net#a] + C[Net#a])) ==> (SqnCh[Net#a][idx$] == idx$)
+  );
+  assert {:msg "  40.15: Channel invariant might not hold on action entry (#9)"} SqnAct[Net#spl] == R[Net#a];
+  assert {:msg "  41.15: Channel invariant might not hold on action entry (#10)"} SqnAct[Net#pri] == R[Net#b];
+  assert {:msg "  42.15: Channel invariant might not hold on action entry (#11)"} SqnAct[Net#sec] == R[Net#c];
+  assert {:msg "  43.15: Channel invariant might not hold on action entry (#12)"} SqnAct[Net#adj] == R[Net#e];
+  assert {:msg "  45.16: Channel invariant might not hold on action entry (#13)"} (forall i: int :: 
+    (0 <= i) && (i < (R[Net#a] + C[Net#a])) ==> (SqnCh[Net#a][i] == i)
+  );
+  assert {:msg "  46.16: Channel invariant might not hold on action entry (#14)"} (forall i: int :: 
+    (0 <= i) && (i < (R[Net#b] + C[Net#b])) ==> (SqnCh[Net#b][i] == i)
+  );
+  assert {:msg "  47.16: Channel invariant might not hold on action entry (#15)"} (forall i: int :: 
+    (0 <= i) && (i < (R[Net#c] + C[Net#c])) ==> (SqnCh[Net#c][i] == i)
+  );
+  assert {:msg "  48.16: Channel invariant might not hold on action entry (#16)"} (forall i: int :: 
+    (0 <= i) && (i < (R[Net#d] + C[Net#d])) ==> (SqnCh[Net#d][i] == i)
+  );
+  assert {:msg "  49.16: Channel invariant might not hold on action entry (#17)"} (forall i: int :: 
+    (0 <= i) && (i < (R[Net#e] + C[Net#e])) ==> (SqnCh[Net#e][i] == i)
+  );
+  assert {:msg "  50.16: Channel invariant might not hold on action entry (#18)"} (forall i: int :: 
+    (0 <= i) && (i < (R[Net#g] + C[Net#g])) ==> (SqnCh[Net#g][i] == i)
+  );
+  assert {:msg "  52.15: Channel invariant might not hold on action entry (#19)"} C[Net#f] == 1;
+  assert {:msg "  53.15: Channel invariant might not hold on action entry (#20)"} (R[Net#g] + C[Net#g]) == R[Net#e];
+  assert {:msg "  54.15: Channel invariant might not hold on action entry (#21)"} R[Net#e] == M[Net#f][R[Net#f]];
+  assert {:msg "  55.16: Channel invariant might not hold on action entry (#22)"} (forall i: int :: 
+    (0 <= i) && (i < (R[Net#g] + C[Net#g])) ==> (SqnCh[Net#g][i] == i)
+  );
+  if ((0 < R[Net#d]) && (0 < R[Net#e])) {
+    assert {:msg "  57.42: Channel invariant might not hold on action entry (#23)"} M[Net#d][R[Net#d] - 1] <= M[Net#e][R[Net#e] - 1];
+  }
+  assert {:msg "  58.16: Channel invariant might not hold on action entry (#24)"} (forall i: int :: 
     (0 <= i) && (i < R[Net#e]) ==> (M[Net#g][i] == M[Net#e][i])
   );
 }
@@ -242,54 +341,107 @@ procedure Net#anon$3#Split#anon$1#8()
   assume 0 <= C[Net#g];
   assume R[Net#g] == 0;
   assume R[Net#a] == (R[Net#b] + C[Net#b]);
+  assert {:msg "  "} R[Net#a] == (R[Net#b] + C[Net#b]);
   assume R[Net#a] == (R[Net#c] + C[Net#c]);
+  assert {:msg "  "} R[Net#a] == (R[Net#c] + C[Net#c]);
   assume R[Net#b] == (R[Net#d] + C[Net#d]);
+  assert {:msg "  "} R[Net#b] == (R[Net#d] + C[Net#d]);
   assume R[Net#c] == (R[Net#e] + C[Net#e]);
+  assert {:msg "  "} R[Net#c] == (R[Net#e] + C[Net#e]);
   assume (forall idx$: int :: 
+    (0 <= idx$) && (idx$ < (R[Net#b] + C[Net#b])) ==> (M[Net#b][idx$] == M[Net#a][idx$])
+  );
+  assert {:msg "  "} (forall idx$: int :: 
     (0 <= idx$) && (idx$ < (R[Net#b] + C[Net#b])) ==> (M[Net#b][idx$] == M[Net#a][idx$])
   );
   assume (forall idx$: int :: 
     (0 <= idx$) && (idx$ < (R[Net#c] + C[Net#c])) ==> (M[Net#c][idx$] == M[Net#a][idx$])
   );
+  assert {:msg "  "} (forall idx$: int :: 
+    (0 <= idx$) && (idx$ < (R[Net#c] + C[Net#c])) ==> (M[Net#c][idx$] == M[Net#a][idx$])
+  );
   assume (forall idx$: int :: 
+    (0 <= idx$) && (idx$ < (R[Net#d] + C[Net#d])) ==> (M[Net#d][idx$] == M[Net#b][idx$])
+  );
+  assert {:msg "  "} (forall idx$: int :: 
     (0 <= idx$) && (idx$ < (R[Net#d] + C[Net#d])) ==> (M[Net#d][idx$] == M[Net#b][idx$])
   );
   assume (forall idx$: int :: 
     (0 <= idx$) && (idx$ < (R[Net#e] + C[Net#e])) ==> (M[Net#e][idx$] == M[Net#c][idx$])
   );
+  assert {:msg "  "} (forall idx$: int :: 
+    (0 <= idx$) && (idx$ < (R[Net#e] + C[Net#e])) ==> (M[Net#e][idx$] == M[Net#c][idx$])
+  );
   assume (forall idx$: int :: 
     (0 <= idx$) && (idx$ < (R[Net#a] + C[Net#a])) ==> (SqnCh[Net#a][idx$] == idx$)
   );
+  assert {:msg "  "} (forall idx$: int :: 
+    (0 <= idx$) && (idx$ < (R[Net#a] + C[Net#a])) ==> (SqnCh[Net#a][idx$] == idx$)
+  );
   assume SqnAct[Net#spl] == R[Net#a];
+  assert {:msg "  40.15: "} SqnAct[Net#spl] == R[Net#a];
   assume SqnAct[Net#pri] == R[Net#b];
+  assert {:msg "  41.15: "} SqnAct[Net#pri] == R[Net#b];
   assume SqnAct[Net#sec] == R[Net#c];
+  assert {:msg "  42.15: "} SqnAct[Net#sec] == R[Net#c];
   assume SqnAct[Net#adj] == R[Net#e];
+  assert {:msg "  43.15: "} SqnAct[Net#adj] == R[Net#e];
   assume (forall i: int :: 
+    (0 <= i) && (i < (R[Net#a] + C[Net#a])) ==> (SqnCh[Net#a][i] == i)
+  );
+  assert {:msg "  45.16: "} (forall i: int :: 
     (0 <= i) && (i < (R[Net#a] + C[Net#a])) ==> (SqnCh[Net#a][i] == i)
   );
   assume (forall i: int :: 
     (0 <= i) && (i < (R[Net#b] + C[Net#b])) ==> (SqnCh[Net#b][i] == i)
   );
+  assert {:msg "  46.16: "} (forall i: int :: 
+    (0 <= i) && (i < (R[Net#b] + C[Net#b])) ==> (SqnCh[Net#b][i] == i)
+  );
   assume (forall i: int :: 
+    (0 <= i) && (i < (R[Net#c] + C[Net#c])) ==> (SqnCh[Net#c][i] == i)
+  );
+  assert {:msg "  47.16: "} (forall i: int :: 
     (0 <= i) && (i < (R[Net#c] + C[Net#c])) ==> (SqnCh[Net#c][i] == i)
   );
   assume (forall i: int :: 
     (0 <= i) && (i < (R[Net#d] + C[Net#d])) ==> (SqnCh[Net#d][i] == i)
   );
+  assert {:msg "  48.16: "} (forall i: int :: 
+    (0 <= i) && (i < (R[Net#d] + C[Net#d])) ==> (SqnCh[Net#d][i] == i)
+  );
   assume (forall i: int :: 
+    (0 <= i) && (i < (R[Net#e] + C[Net#e])) ==> (SqnCh[Net#e][i] == i)
+  );
+  assert {:msg "  49.16: "} (forall i: int :: 
     (0 <= i) && (i < (R[Net#e] + C[Net#e])) ==> (SqnCh[Net#e][i] == i)
   );
   assume (forall i: int :: 
     (0 <= i) && (i < (R[Net#g] + C[Net#g])) ==> (SqnCh[Net#g][i] == i)
   );
+  assert {:msg "  50.16: "} (forall i: int :: 
+    (0 <= i) && (i < (R[Net#g] + C[Net#g])) ==> (SqnCh[Net#g][i] == i)
+  );
   assume C[Net#f] == 1;
-  assume C[Net#g] == R[Net#e];
+  assert {:msg "  52.15: "} C[Net#f] == 1;
+  assume (R[Net#g] + C[Net#g]) == R[Net#e];
+  assert {:msg "  53.15: "} (R[Net#g] + C[Net#g]) == R[Net#e];
   assume R[Net#e] == M[Net#f][R[Net#f]];
+  assert {:msg "  54.15: "} R[Net#e] == M[Net#f][R[Net#f]];
   assume (forall i: int :: 
     (0 <= i) && (i < (R[Net#g] + C[Net#g])) ==> (SqnCh[Net#g][i] == i)
   );
-  assume (0 < R[Net#d]) && (0 < R[Net#e]) ==> (M[Net#d][R[Net#d] - 1] <= M[Net#e][R[Net#e] - 1]);
+  assert {:msg "  55.16: "} (forall i: int :: 
+    (0 <= i) && (i < (R[Net#g] + C[Net#g])) ==> (SqnCh[Net#g][i] == i)
+  );
+  if ((0 < R[Net#d]) && (0 < R[Net#e])) {
+    assume M[Net#d][R[Net#d] - 1] <= M[Net#e][R[Net#e] - 1];
+    assert {:msg "  57.42: "} M[Net#d][R[Net#d] - 1] <= M[Net#e][R[Net#e] - 1];
+  }
   assume (forall i: int :: 
+    (0 <= i) && (i < R[Net#e]) ==> (M[Net#g][i] == M[Net#e][i])
+  );
+  assert {:msg "  58.16: "} (forall i: int :: 
     (0 <= i) && (i < R[Net#e]) ==> (M[Net#g][i] == M[Net#e][i])
   );
   assume true;
@@ -304,71 +456,57 @@ procedure Net#anon$3#Split#anon$1#8()
   SqnCh[Net#c][R[Net#c] + C[Net#c]] := SqnAct[Net#spl];
   C[Net#c] := C[Net#c] + 1;
   SqnAct[Net#spl] := SqnAct[Net#spl] + 1;
-  assume 0 <= R[Net#a];
-  assume 0 <= C[Net#a];
-  assume (R[Net#a] + C[Net#a]) <= L[Net#a];
-  assume 0 <= R[Net#b];
-  assume 0 <= C[Net#b];
-  assume 0 <= R[Net#c];
-  assume 0 <= C[Net#c];
-  assume 0 <= R[Net#d];
-  assume 0 <= C[Net#d];
-  assume 0 <= R[Net#e];
-  assume 0 <= C[Net#e];
-  assume 0 <= R[Net#f];
-  assume 0 <= C[Net#f];
-  assume 0 <= R[Net#g];
-  assume 0 <= C[Net#g];
-  assume R[Net#g] == 0;
-  assert {:msg "  Action at 8.3 ('anon$1') for actor instance 'spl' might not preserve the channel invariant (#57)"} R[Net#a] == (R[Net#b] + C[Net#b]);
-  assert {:msg "  Action at 8.3 ('anon$1') for actor instance 'spl' might not preserve the channel invariant (#58)"} R[Net#a] == (R[Net#c] + C[Net#c]);
-  assert {:msg "  Action at 8.3 ('anon$1') for actor instance 'spl' might not preserve the channel invariant (#59)"} R[Net#b] == (R[Net#d] + C[Net#d]);
-  assert {:msg "  Action at 8.3 ('anon$1') for actor instance 'spl' might not preserve the channel invariant (#60)"} R[Net#c] == (R[Net#e] + C[Net#e]);
-  assert {:msg "  Action at 8.3 ('anon$1') for actor instance 'spl' might not preserve the channel invariant (#61)"} (forall idx$: int :: 
+  assert {:msg "  Action at 8.3 ('anon$1') for actor instance 'spl' might not preserve the channel invariant (#25)"} R[Net#a] == (R[Net#b] + C[Net#b]);
+  assert {:msg "  Action at 8.3 ('anon$1') for actor instance 'spl' might not preserve the channel invariant (#26)"} R[Net#a] == (R[Net#c] + C[Net#c]);
+  assert {:msg "  Action at 8.3 ('anon$1') for actor instance 'spl' might not preserve the channel invariant (#27)"} R[Net#b] == (R[Net#d] + C[Net#d]);
+  assert {:msg "  Action at 8.3 ('anon$1') for actor instance 'spl' might not preserve the channel invariant (#28)"} R[Net#c] == (R[Net#e] + C[Net#e]);
+  assert {:msg "  Action at 8.3 ('anon$1') for actor instance 'spl' might not preserve the channel invariant (#29)"} (forall idx$: int :: 
     (0 <= idx$) && (idx$ < (R[Net#b] + C[Net#b])) ==> (M[Net#b][idx$] == M[Net#a][idx$])
   );
-  assert {:msg "  Action at 8.3 ('anon$1') for actor instance 'spl' might not preserve the channel invariant (#62)"} (forall idx$: int :: 
+  assert {:msg "  Action at 8.3 ('anon$1') for actor instance 'spl' might not preserve the channel invariant (#30)"} (forall idx$: int :: 
     (0 <= idx$) && (idx$ < (R[Net#c] + C[Net#c])) ==> (M[Net#c][idx$] == M[Net#a][idx$])
   );
-  assert {:msg "  Action at 8.3 ('anon$1') for actor instance 'spl' might not preserve the channel invariant (#63)"} (forall idx$: int :: 
+  assert {:msg "  Action at 8.3 ('anon$1') for actor instance 'spl' might not preserve the channel invariant (#31)"} (forall idx$: int :: 
     (0 <= idx$) && (idx$ < (R[Net#d] + C[Net#d])) ==> (M[Net#d][idx$] == M[Net#b][idx$])
   );
-  assert {:msg "  Action at 8.3 ('anon$1') for actor instance 'spl' might not preserve the channel invariant (#64)"} (forall idx$: int :: 
+  assert {:msg "  Action at 8.3 ('anon$1') for actor instance 'spl' might not preserve the channel invariant (#32)"} (forall idx$: int :: 
     (0 <= idx$) && (idx$ < (R[Net#e] + C[Net#e])) ==> (M[Net#e][idx$] == M[Net#c][idx$])
   );
-  assert {:msg "  Action at 8.3 ('anon$1') for actor instance 'spl' might not preserve the channel invariant (#65)"} (forall idx$: int :: 
+  assert {:msg "  Action at 8.3 ('anon$1') for actor instance 'spl' might not preserve the channel invariant (#33)"} (forall idx$: int :: 
     (0 <= idx$) && (idx$ < (R[Net#a] + C[Net#a])) ==> (SqnCh[Net#a][idx$] == idx$)
   );
-  assert {:msg "  40.3: Action at 8.3 ('anon$1') for actor instance 'spl' might not preserve the channel invariant (#66)"} SqnAct[Net#spl] == R[Net#a];
-  assert {:msg "  41.3: Action at 8.3 ('anon$1') for actor instance 'spl' might not preserve the channel invariant (#67)"} SqnAct[Net#pri] == R[Net#b];
-  assert {:msg "  42.3: Action at 8.3 ('anon$1') for actor instance 'spl' might not preserve the channel invariant (#68)"} SqnAct[Net#sec] == R[Net#c];
-  assert {:msg "  43.3: Action at 8.3 ('anon$1') for actor instance 'spl' might not preserve the channel invariant (#69)"} SqnAct[Net#adj] == R[Net#e];
-  assert {:msg "  45.3: Action at 8.3 ('anon$1') for actor instance 'spl' might not preserve the channel invariant (#70)"} (forall i: int :: 
+  assert {:msg "  40.15: Action at 8.3 ('anon$1') for actor instance 'spl' might not preserve the channel invariant (#34)"} SqnAct[Net#spl] == R[Net#a];
+  assert {:msg "  41.15: Action at 8.3 ('anon$1') for actor instance 'spl' might not preserve the channel invariant (#35)"} SqnAct[Net#pri] == R[Net#b];
+  assert {:msg "  42.15: Action at 8.3 ('anon$1') for actor instance 'spl' might not preserve the channel invariant (#36)"} SqnAct[Net#sec] == R[Net#c];
+  assert {:msg "  43.15: Action at 8.3 ('anon$1') for actor instance 'spl' might not preserve the channel invariant (#37)"} SqnAct[Net#adj] == R[Net#e];
+  assert {:msg "  45.16: Action at 8.3 ('anon$1') for actor instance 'spl' might not preserve the channel invariant (#38)"} (forall i: int :: 
     (0 <= i) && (i < (R[Net#a] + C[Net#a])) ==> (SqnCh[Net#a][i] == i)
   );
-  assert {:msg "  46.3: Action at 8.3 ('anon$1') for actor instance 'spl' might not preserve the channel invariant (#71)"} (forall i: int :: 
+  assert {:msg "  46.16: Action at 8.3 ('anon$1') for actor instance 'spl' might not preserve the channel invariant (#39)"} (forall i: int :: 
     (0 <= i) && (i < (R[Net#b] + C[Net#b])) ==> (SqnCh[Net#b][i] == i)
   );
-  assert {:msg "  47.3: Action at 8.3 ('anon$1') for actor instance 'spl' might not preserve the channel invariant (#72)"} (forall i: int :: 
+  assert {:msg "  47.16: Action at 8.3 ('anon$1') for actor instance 'spl' might not preserve the channel invariant (#40)"} (forall i: int :: 
     (0 <= i) && (i < (R[Net#c] + C[Net#c])) ==> (SqnCh[Net#c][i] == i)
   );
-  assert {:msg "  48.3: Action at 8.3 ('anon$1') for actor instance 'spl' might not preserve the channel invariant (#73)"} (forall i: int :: 
+  assert {:msg "  48.16: Action at 8.3 ('anon$1') for actor instance 'spl' might not preserve the channel invariant (#41)"} (forall i: int :: 
     (0 <= i) && (i < (R[Net#d] + C[Net#d])) ==> (SqnCh[Net#d][i] == i)
   );
-  assert {:msg "  49.3: Action at 8.3 ('anon$1') for actor instance 'spl' might not preserve the channel invariant (#74)"} (forall i: int :: 
+  assert {:msg "  49.16: Action at 8.3 ('anon$1') for actor instance 'spl' might not preserve the channel invariant (#42)"} (forall i: int :: 
     (0 <= i) && (i < (R[Net#e] + C[Net#e])) ==> (SqnCh[Net#e][i] == i)
   );
-  assert {:msg "  50.3: Action at 8.3 ('anon$1') for actor instance 'spl' might not preserve the channel invariant (#75)"} (forall i: int :: 
+  assert {:msg "  50.16: Action at 8.3 ('anon$1') for actor instance 'spl' might not preserve the channel invariant (#43)"} (forall i: int :: 
     (0 <= i) && (i < (R[Net#g] + C[Net#g])) ==> (SqnCh[Net#g][i] == i)
   );
-  assert {:msg "  52.3: Action at 8.3 ('anon$1') for actor instance 'spl' might not preserve the channel invariant (#76)"} C[Net#f] == 1;
-  assert {:msg "  53.3: Action at 8.3 ('anon$1') for actor instance 'spl' might not preserve the channel invariant (#77)"} C[Net#g] == R[Net#e];
-  assert {:msg "  54.3: Action at 8.3 ('anon$1') for actor instance 'spl' might not preserve the channel invariant (#78)"} R[Net#e] == M[Net#f][R[Net#f]];
-  assert {:msg "  55.3: Action at 8.3 ('anon$1') for actor instance 'spl' might not preserve the channel invariant (#79)"} (forall i: int :: 
+  assert {:msg "  52.15: Action at 8.3 ('anon$1') for actor instance 'spl' might not preserve the channel invariant (#44)"} C[Net#f] == 1;
+  assert {:msg "  53.15: Action at 8.3 ('anon$1') for actor instance 'spl' might not preserve the channel invariant (#45)"} (R[Net#g] + C[Net#g]) == R[Net#e];
+  assert {:msg "  54.15: Action at 8.3 ('anon$1') for actor instance 'spl' might not preserve the channel invariant (#46)"} R[Net#e] == M[Net#f][R[Net#f]];
+  assert {:msg "  55.16: Action at 8.3 ('anon$1') for actor instance 'spl' might not preserve the channel invariant (#47)"} (forall i: int :: 
     (0 <= i) && (i < (R[Net#g] + C[Net#g])) ==> (SqnCh[Net#g][i] == i)
   );
-  assert {:msg "  59.3: Action at 8.3 ('anon$1') for actor instance 'spl' might not preserve the channel invariant (#80)"} (0 < R[Net#d]) && (0 < R[Net#e]) ==> (M[Net#d][R[Net#d] - 1] <= M[Net#e][R[Net#e] - 1]);
-  assert {:msg "  60.3: Action at 8.3 ('anon$1') for actor instance 'spl' might not preserve the channel invariant (#81)"} (forall i: int :: 
+  if ((0 < R[Net#d]) && (0 < R[Net#e])) {
+    assert {:msg "  57.42: Action at 8.3 ('anon$1') for actor instance 'spl' might not preserve the channel invariant (#48)"} M[Net#d][R[Net#d] - 1] <= M[Net#e][R[Net#e] - 1];
+  }
+  assert {:msg "  58.16: Action at 8.3 ('anon$1') for actor instance 'spl' might not preserve the channel invariant (#49)"} (forall i: int :: 
     (0 <= i) && (i < R[Net#e]) ==> (M[Net#g][i] == M[Net#e][i])
   );
 }
@@ -395,54 +533,107 @@ procedure Net#anon$3#Rep#anon$0#9()
   assume 0 <= C[Net#g];
   assume R[Net#g] == 0;
   assume R[Net#a] == (R[Net#b] + C[Net#b]);
+  assert {:msg "  "} R[Net#a] == (R[Net#b] + C[Net#b]);
   assume R[Net#a] == (R[Net#c] + C[Net#c]);
+  assert {:msg "  "} R[Net#a] == (R[Net#c] + C[Net#c]);
   assume R[Net#b] == (R[Net#d] + C[Net#d]);
+  assert {:msg "  "} R[Net#b] == (R[Net#d] + C[Net#d]);
   assume R[Net#c] == (R[Net#e] + C[Net#e]);
+  assert {:msg "  "} R[Net#c] == (R[Net#e] + C[Net#e]);
   assume (forall idx$: int :: 
+    (0 <= idx$) && (idx$ < (R[Net#b] + C[Net#b])) ==> (M[Net#b][idx$] == M[Net#a][idx$])
+  );
+  assert {:msg "  "} (forall idx$: int :: 
     (0 <= idx$) && (idx$ < (R[Net#b] + C[Net#b])) ==> (M[Net#b][idx$] == M[Net#a][idx$])
   );
   assume (forall idx$: int :: 
     (0 <= idx$) && (idx$ < (R[Net#c] + C[Net#c])) ==> (M[Net#c][idx$] == M[Net#a][idx$])
   );
+  assert {:msg "  "} (forall idx$: int :: 
+    (0 <= idx$) && (idx$ < (R[Net#c] + C[Net#c])) ==> (M[Net#c][idx$] == M[Net#a][idx$])
+  );
   assume (forall idx$: int :: 
+    (0 <= idx$) && (idx$ < (R[Net#d] + C[Net#d])) ==> (M[Net#d][idx$] == M[Net#b][idx$])
+  );
+  assert {:msg "  "} (forall idx$: int :: 
     (0 <= idx$) && (idx$ < (R[Net#d] + C[Net#d])) ==> (M[Net#d][idx$] == M[Net#b][idx$])
   );
   assume (forall idx$: int :: 
     (0 <= idx$) && (idx$ < (R[Net#e] + C[Net#e])) ==> (M[Net#e][idx$] == M[Net#c][idx$])
   );
+  assert {:msg "  "} (forall idx$: int :: 
+    (0 <= idx$) && (idx$ < (R[Net#e] + C[Net#e])) ==> (M[Net#e][idx$] == M[Net#c][idx$])
+  );
   assume (forall idx$: int :: 
     (0 <= idx$) && (idx$ < (R[Net#a] + C[Net#a])) ==> (SqnCh[Net#a][idx$] == idx$)
   );
+  assert {:msg "  "} (forall idx$: int :: 
+    (0 <= idx$) && (idx$ < (R[Net#a] + C[Net#a])) ==> (SqnCh[Net#a][idx$] == idx$)
+  );
   assume SqnAct[Net#spl] == R[Net#a];
+  assert {:msg "  40.15: "} SqnAct[Net#spl] == R[Net#a];
   assume SqnAct[Net#pri] == R[Net#b];
+  assert {:msg "  41.15: "} SqnAct[Net#pri] == R[Net#b];
   assume SqnAct[Net#sec] == R[Net#c];
+  assert {:msg "  42.15: "} SqnAct[Net#sec] == R[Net#c];
   assume SqnAct[Net#adj] == R[Net#e];
+  assert {:msg "  43.15: "} SqnAct[Net#adj] == R[Net#e];
   assume (forall i: int :: 
+    (0 <= i) && (i < (R[Net#a] + C[Net#a])) ==> (SqnCh[Net#a][i] == i)
+  );
+  assert {:msg "  45.16: "} (forall i: int :: 
     (0 <= i) && (i < (R[Net#a] + C[Net#a])) ==> (SqnCh[Net#a][i] == i)
   );
   assume (forall i: int :: 
     (0 <= i) && (i < (R[Net#b] + C[Net#b])) ==> (SqnCh[Net#b][i] == i)
   );
+  assert {:msg "  46.16: "} (forall i: int :: 
+    (0 <= i) && (i < (R[Net#b] + C[Net#b])) ==> (SqnCh[Net#b][i] == i)
+  );
   assume (forall i: int :: 
+    (0 <= i) && (i < (R[Net#c] + C[Net#c])) ==> (SqnCh[Net#c][i] == i)
+  );
+  assert {:msg "  47.16: "} (forall i: int :: 
     (0 <= i) && (i < (R[Net#c] + C[Net#c])) ==> (SqnCh[Net#c][i] == i)
   );
   assume (forall i: int :: 
     (0 <= i) && (i < (R[Net#d] + C[Net#d])) ==> (SqnCh[Net#d][i] == i)
   );
+  assert {:msg "  48.16: "} (forall i: int :: 
+    (0 <= i) && (i < (R[Net#d] + C[Net#d])) ==> (SqnCh[Net#d][i] == i)
+  );
   assume (forall i: int :: 
+    (0 <= i) && (i < (R[Net#e] + C[Net#e])) ==> (SqnCh[Net#e][i] == i)
+  );
+  assert {:msg "  49.16: "} (forall i: int :: 
     (0 <= i) && (i < (R[Net#e] + C[Net#e])) ==> (SqnCh[Net#e][i] == i)
   );
   assume (forall i: int :: 
     (0 <= i) && (i < (R[Net#g] + C[Net#g])) ==> (SqnCh[Net#g][i] == i)
   );
+  assert {:msg "  50.16: "} (forall i: int :: 
+    (0 <= i) && (i < (R[Net#g] + C[Net#g])) ==> (SqnCh[Net#g][i] == i)
+  );
   assume C[Net#f] == 1;
-  assume C[Net#g] == R[Net#e];
+  assert {:msg "  52.15: "} C[Net#f] == 1;
+  assume (R[Net#g] + C[Net#g]) == R[Net#e];
+  assert {:msg "  53.15: "} (R[Net#g] + C[Net#g]) == R[Net#e];
   assume R[Net#e] == M[Net#f][R[Net#f]];
+  assert {:msg "  54.15: "} R[Net#e] == M[Net#f][R[Net#f]];
   assume (forall i: int :: 
     (0 <= i) && (i < (R[Net#g] + C[Net#g])) ==> (SqnCh[Net#g][i] == i)
   );
-  assume (0 < R[Net#d]) && (0 < R[Net#e]) ==> (M[Net#d][R[Net#d] - 1] <= M[Net#e][R[Net#e] - 1]);
+  assert {:msg "  55.16: "} (forall i: int :: 
+    (0 <= i) && (i < (R[Net#g] + C[Net#g])) ==> (SqnCh[Net#g][i] == i)
+  );
+  if ((0 < R[Net#d]) && (0 < R[Net#e])) {
+    assume M[Net#d][R[Net#d] - 1] <= M[Net#e][R[Net#e] - 1];
+    assert {:msg "  57.42: "} M[Net#d][R[Net#d] - 1] <= M[Net#e][R[Net#e] - 1];
+  }
   assume (forall i: int :: 
+    (0 <= i) && (i < R[Net#e]) ==> (M[Net#g][i] == M[Net#e][i])
+  );
+  assert {:msg "  58.16: "} (forall i: int :: 
     (0 <= i) && (i < R[Net#e]) ==> (M[Net#g][i] == M[Net#e][i])
   );
   assume true;
@@ -454,71 +645,57 @@ procedure Net#anon$3#Rep#anon$0#9()
   SqnCh[Net#d][R[Net#d] + C[Net#d]] := SqnAct[Net#pri];
   C[Net#d] := C[Net#d] + 1;
   SqnAct[Net#pri] := SqnAct[Net#pri] + 1;
-  assume 0 <= R[Net#a];
-  assume 0 <= C[Net#a];
-  assume (R[Net#a] + C[Net#a]) <= L[Net#a];
-  assume 0 <= R[Net#b];
-  assume 0 <= C[Net#b];
-  assume 0 <= R[Net#c];
-  assume 0 <= C[Net#c];
-  assume 0 <= R[Net#d];
-  assume 0 <= C[Net#d];
-  assume 0 <= R[Net#e];
-  assume 0 <= C[Net#e];
-  assume 0 <= R[Net#f];
-  assume 0 <= C[Net#f];
-  assume 0 <= R[Net#g];
-  assume 0 <= C[Net#g];
-  assume R[Net#g] == 0;
-  assert {:msg "  Action at 3.3 ('anon$0') for actor instance 'pri' might not preserve the channel invariant (#98)"} R[Net#a] == (R[Net#b] + C[Net#b]);
-  assert {:msg "  Action at 3.3 ('anon$0') for actor instance 'pri' might not preserve the channel invariant (#99)"} R[Net#a] == (R[Net#c] + C[Net#c]);
-  assert {:msg "  Action at 3.3 ('anon$0') for actor instance 'pri' might not preserve the channel invariant (#100)"} R[Net#b] == (R[Net#d] + C[Net#d]);
-  assert {:msg "  Action at 3.3 ('anon$0') for actor instance 'pri' might not preserve the channel invariant (#101)"} R[Net#c] == (R[Net#e] + C[Net#e]);
-  assert {:msg "  Action at 3.3 ('anon$0') for actor instance 'pri' might not preserve the channel invariant (#102)"} (forall idx$: int :: 
+  assert {:msg "  Action at 3.3 ('anon$0') for actor instance 'pri' might not preserve the channel invariant (#50)"} R[Net#a] == (R[Net#b] + C[Net#b]);
+  assert {:msg "  Action at 3.3 ('anon$0') for actor instance 'pri' might not preserve the channel invariant (#51)"} R[Net#a] == (R[Net#c] + C[Net#c]);
+  assert {:msg "  Action at 3.3 ('anon$0') for actor instance 'pri' might not preserve the channel invariant (#52)"} R[Net#b] == (R[Net#d] + C[Net#d]);
+  assert {:msg "  Action at 3.3 ('anon$0') for actor instance 'pri' might not preserve the channel invariant (#53)"} R[Net#c] == (R[Net#e] + C[Net#e]);
+  assert {:msg "  Action at 3.3 ('anon$0') for actor instance 'pri' might not preserve the channel invariant (#54)"} (forall idx$: int :: 
     (0 <= idx$) && (idx$ < (R[Net#b] + C[Net#b])) ==> (M[Net#b][idx$] == M[Net#a][idx$])
   );
-  assert {:msg "  Action at 3.3 ('anon$0') for actor instance 'pri' might not preserve the channel invariant (#103)"} (forall idx$: int :: 
+  assert {:msg "  Action at 3.3 ('anon$0') for actor instance 'pri' might not preserve the channel invariant (#55)"} (forall idx$: int :: 
     (0 <= idx$) && (idx$ < (R[Net#c] + C[Net#c])) ==> (M[Net#c][idx$] == M[Net#a][idx$])
   );
-  assert {:msg "  Action at 3.3 ('anon$0') for actor instance 'pri' might not preserve the channel invariant (#104)"} (forall idx$: int :: 
+  assert {:msg "  Action at 3.3 ('anon$0') for actor instance 'pri' might not preserve the channel invariant (#56)"} (forall idx$: int :: 
     (0 <= idx$) && (idx$ < (R[Net#d] + C[Net#d])) ==> (M[Net#d][idx$] == M[Net#b][idx$])
   );
-  assert {:msg "  Action at 3.3 ('anon$0') for actor instance 'pri' might not preserve the channel invariant (#105)"} (forall idx$: int :: 
+  assert {:msg "  Action at 3.3 ('anon$0') for actor instance 'pri' might not preserve the channel invariant (#57)"} (forall idx$: int :: 
     (0 <= idx$) && (idx$ < (R[Net#e] + C[Net#e])) ==> (M[Net#e][idx$] == M[Net#c][idx$])
   );
-  assert {:msg "  Action at 3.3 ('anon$0') for actor instance 'pri' might not preserve the channel invariant (#106)"} (forall idx$: int :: 
+  assert {:msg "  Action at 3.3 ('anon$0') for actor instance 'pri' might not preserve the channel invariant (#58)"} (forall idx$: int :: 
     (0 <= idx$) && (idx$ < (R[Net#a] + C[Net#a])) ==> (SqnCh[Net#a][idx$] == idx$)
   );
-  assert {:msg "  40.3: Action at 3.3 ('anon$0') for actor instance 'pri' might not preserve the channel invariant (#107)"} SqnAct[Net#spl] == R[Net#a];
-  assert {:msg "  41.3: Action at 3.3 ('anon$0') for actor instance 'pri' might not preserve the channel invariant (#108)"} SqnAct[Net#pri] == R[Net#b];
-  assert {:msg "  42.3: Action at 3.3 ('anon$0') for actor instance 'pri' might not preserve the channel invariant (#109)"} SqnAct[Net#sec] == R[Net#c];
-  assert {:msg "  43.3: Action at 3.3 ('anon$0') for actor instance 'pri' might not preserve the channel invariant (#110)"} SqnAct[Net#adj] == R[Net#e];
-  assert {:msg "  45.3: Action at 3.3 ('anon$0') for actor instance 'pri' might not preserve the channel invariant (#111)"} (forall i: int :: 
+  assert {:msg "  40.15: Action at 3.3 ('anon$0') for actor instance 'pri' might not preserve the channel invariant (#59)"} SqnAct[Net#spl] == R[Net#a];
+  assert {:msg "  41.15: Action at 3.3 ('anon$0') for actor instance 'pri' might not preserve the channel invariant (#60)"} SqnAct[Net#pri] == R[Net#b];
+  assert {:msg "  42.15: Action at 3.3 ('anon$0') for actor instance 'pri' might not preserve the channel invariant (#61)"} SqnAct[Net#sec] == R[Net#c];
+  assert {:msg "  43.15: Action at 3.3 ('anon$0') for actor instance 'pri' might not preserve the channel invariant (#62)"} SqnAct[Net#adj] == R[Net#e];
+  assert {:msg "  45.16: Action at 3.3 ('anon$0') for actor instance 'pri' might not preserve the channel invariant (#63)"} (forall i: int :: 
     (0 <= i) && (i < (R[Net#a] + C[Net#a])) ==> (SqnCh[Net#a][i] == i)
   );
-  assert {:msg "  46.3: Action at 3.3 ('anon$0') for actor instance 'pri' might not preserve the channel invariant (#112)"} (forall i: int :: 
+  assert {:msg "  46.16: Action at 3.3 ('anon$0') for actor instance 'pri' might not preserve the channel invariant (#64)"} (forall i: int :: 
     (0 <= i) && (i < (R[Net#b] + C[Net#b])) ==> (SqnCh[Net#b][i] == i)
   );
-  assert {:msg "  47.3: Action at 3.3 ('anon$0') for actor instance 'pri' might not preserve the channel invariant (#113)"} (forall i: int :: 
+  assert {:msg "  47.16: Action at 3.3 ('anon$0') for actor instance 'pri' might not preserve the channel invariant (#65)"} (forall i: int :: 
     (0 <= i) && (i < (R[Net#c] + C[Net#c])) ==> (SqnCh[Net#c][i] == i)
   );
-  assert {:msg "  48.3: Action at 3.3 ('anon$0') for actor instance 'pri' might not preserve the channel invariant (#114)"} (forall i: int :: 
+  assert {:msg "  48.16: Action at 3.3 ('anon$0') for actor instance 'pri' might not preserve the channel invariant (#66)"} (forall i: int :: 
     (0 <= i) && (i < (R[Net#d] + C[Net#d])) ==> (SqnCh[Net#d][i] == i)
   );
-  assert {:msg "  49.3: Action at 3.3 ('anon$0') for actor instance 'pri' might not preserve the channel invariant (#115)"} (forall i: int :: 
+  assert {:msg "  49.16: Action at 3.3 ('anon$0') for actor instance 'pri' might not preserve the channel invariant (#67)"} (forall i: int :: 
     (0 <= i) && (i < (R[Net#e] + C[Net#e])) ==> (SqnCh[Net#e][i] == i)
   );
-  assert {:msg "  50.3: Action at 3.3 ('anon$0') for actor instance 'pri' might not preserve the channel invariant (#116)"} (forall i: int :: 
+  assert {:msg "  50.16: Action at 3.3 ('anon$0') for actor instance 'pri' might not preserve the channel invariant (#68)"} (forall i: int :: 
     (0 <= i) && (i < (R[Net#g] + C[Net#g])) ==> (SqnCh[Net#g][i] == i)
   );
-  assert {:msg "  52.3: Action at 3.3 ('anon$0') for actor instance 'pri' might not preserve the channel invariant (#117)"} C[Net#f] == 1;
-  assert {:msg "  53.3: Action at 3.3 ('anon$0') for actor instance 'pri' might not preserve the channel invariant (#118)"} C[Net#g] == R[Net#e];
-  assert {:msg "  54.3: Action at 3.3 ('anon$0') for actor instance 'pri' might not preserve the channel invariant (#119)"} R[Net#e] == M[Net#f][R[Net#f]];
-  assert {:msg "  55.3: Action at 3.3 ('anon$0') for actor instance 'pri' might not preserve the channel invariant (#120)"} (forall i: int :: 
+  assert {:msg "  52.15: Action at 3.3 ('anon$0') for actor instance 'pri' might not preserve the channel invariant (#69)"} C[Net#f] == 1;
+  assert {:msg "  53.15: Action at 3.3 ('anon$0') for actor instance 'pri' might not preserve the channel invariant (#70)"} (R[Net#g] + C[Net#g]) == R[Net#e];
+  assert {:msg "  54.15: Action at 3.3 ('anon$0') for actor instance 'pri' might not preserve the channel invariant (#71)"} R[Net#e] == M[Net#f][R[Net#f]];
+  assert {:msg "  55.16: Action at 3.3 ('anon$0') for actor instance 'pri' might not preserve the channel invariant (#72)"} (forall i: int :: 
     (0 <= i) && (i < (R[Net#g] + C[Net#g])) ==> (SqnCh[Net#g][i] == i)
   );
-  assert {:msg "  59.3: Action at 3.3 ('anon$0') for actor instance 'pri' might not preserve the channel invariant (#121)"} (0 < R[Net#d]) && (0 < R[Net#e]) ==> (M[Net#d][R[Net#d] - 1] <= M[Net#e][R[Net#e] - 1]);
-  assert {:msg "  60.3: Action at 3.3 ('anon$0') for actor instance 'pri' might not preserve the channel invariant (#122)"} (forall i: int :: 
+  if ((0 < R[Net#d]) && (0 < R[Net#e])) {
+    assert {:msg "  57.42: Action at 3.3 ('anon$0') for actor instance 'pri' might not preserve the channel invariant (#73)"} M[Net#d][R[Net#d] - 1] <= M[Net#e][R[Net#e] - 1];
+  }
+  assert {:msg "  58.16: Action at 3.3 ('anon$0') for actor instance 'pri' might not preserve the channel invariant (#74)"} (forall i: int :: 
     (0 <= i) && (i < R[Net#e]) ==> (M[Net#g][i] == M[Net#e][i])
   );
 }
@@ -545,54 +722,107 @@ procedure Net#anon$3#Rep#anon$0#10()
   assume 0 <= C[Net#g];
   assume R[Net#g] == 0;
   assume R[Net#a] == (R[Net#b] + C[Net#b]);
+  assert {:msg "  "} R[Net#a] == (R[Net#b] + C[Net#b]);
   assume R[Net#a] == (R[Net#c] + C[Net#c]);
+  assert {:msg "  "} R[Net#a] == (R[Net#c] + C[Net#c]);
   assume R[Net#b] == (R[Net#d] + C[Net#d]);
+  assert {:msg "  "} R[Net#b] == (R[Net#d] + C[Net#d]);
   assume R[Net#c] == (R[Net#e] + C[Net#e]);
+  assert {:msg "  "} R[Net#c] == (R[Net#e] + C[Net#e]);
   assume (forall idx$: int :: 
+    (0 <= idx$) && (idx$ < (R[Net#b] + C[Net#b])) ==> (M[Net#b][idx$] == M[Net#a][idx$])
+  );
+  assert {:msg "  "} (forall idx$: int :: 
     (0 <= idx$) && (idx$ < (R[Net#b] + C[Net#b])) ==> (M[Net#b][idx$] == M[Net#a][idx$])
   );
   assume (forall idx$: int :: 
     (0 <= idx$) && (idx$ < (R[Net#c] + C[Net#c])) ==> (M[Net#c][idx$] == M[Net#a][idx$])
   );
+  assert {:msg "  "} (forall idx$: int :: 
+    (0 <= idx$) && (idx$ < (R[Net#c] + C[Net#c])) ==> (M[Net#c][idx$] == M[Net#a][idx$])
+  );
   assume (forall idx$: int :: 
+    (0 <= idx$) && (idx$ < (R[Net#d] + C[Net#d])) ==> (M[Net#d][idx$] == M[Net#b][idx$])
+  );
+  assert {:msg "  "} (forall idx$: int :: 
     (0 <= idx$) && (idx$ < (R[Net#d] + C[Net#d])) ==> (M[Net#d][idx$] == M[Net#b][idx$])
   );
   assume (forall idx$: int :: 
     (0 <= idx$) && (idx$ < (R[Net#e] + C[Net#e])) ==> (M[Net#e][idx$] == M[Net#c][idx$])
   );
+  assert {:msg "  "} (forall idx$: int :: 
+    (0 <= idx$) && (idx$ < (R[Net#e] + C[Net#e])) ==> (M[Net#e][idx$] == M[Net#c][idx$])
+  );
   assume (forall idx$: int :: 
     (0 <= idx$) && (idx$ < (R[Net#a] + C[Net#a])) ==> (SqnCh[Net#a][idx$] == idx$)
   );
+  assert {:msg "  "} (forall idx$: int :: 
+    (0 <= idx$) && (idx$ < (R[Net#a] + C[Net#a])) ==> (SqnCh[Net#a][idx$] == idx$)
+  );
   assume SqnAct[Net#spl] == R[Net#a];
+  assert {:msg "  40.15: "} SqnAct[Net#spl] == R[Net#a];
   assume SqnAct[Net#pri] == R[Net#b];
+  assert {:msg "  41.15: "} SqnAct[Net#pri] == R[Net#b];
   assume SqnAct[Net#sec] == R[Net#c];
+  assert {:msg "  42.15: "} SqnAct[Net#sec] == R[Net#c];
   assume SqnAct[Net#adj] == R[Net#e];
+  assert {:msg "  43.15: "} SqnAct[Net#adj] == R[Net#e];
   assume (forall i: int :: 
+    (0 <= i) && (i < (R[Net#a] + C[Net#a])) ==> (SqnCh[Net#a][i] == i)
+  );
+  assert {:msg "  45.16: "} (forall i: int :: 
     (0 <= i) && (i < (R[Net#a] + C[Net#a])) ==> (SqnCh[Net#a][i] == i)
   );
   assume (forall i: int :: 
     (0 <= i) && (i < (R[Net#b] + C[Net#b])) ==> (SqnCh[Net#b][i] == i)
   );
+  assert {:msg "  46.16: "} (forall i: int :: 
+    (0 <= i) && (i < (R[Net#b] + C[Net#b])) ==> (SqnCh[Net#b][i] == i)
+  );
   assume (forall i: int :: 
+    (0 <= i) && (i < (R[Net#c] + C[Net#c])) ==> (SqnCh[Net#c][i] == i)
+  );
+  assert {:msg "  47.16: "} (forall i: int :: 
     (0 <= i) && (i < (R[Net#c] + C[Net#c])) ==> (SqnCh[Net#c][i] == i)
   );
   assume (forall i: int :: 
     (0 <= i) && (i < (R[Net#d] + C[Net#d])) ==> (SqnCh[Net#d][i] == i)
   );
+  assert {:msg "  48.16: "} (forall i: int :: 
+    (0 <= i) && (i < (R[Net#d] + C[Net#d])) ==> (SqnCh[Net#d][i] == i)
+  );
   assume (forall i: int :: 
+    (0 <= i) && (i < (R[Net#e] + C[Net#e])) ==> (SqnCh[Net#e][i] == i)
+  );
+  assert {:msg "  49.16: "} (forall i: int :: 
     (0 <= i) && (i < (R[Net#e] + C[Net#e])) ==> (SqnCh[Net#e][i] == i)
   );
   assume (forall i: int :: 
     (0 <= i) && (i < (R[Net#g] + C[Net#g])) ==> (SqnCh[Net#g][i] == i)
   );
+  assert {:msg "  50.16: "} (forall i: int :: 
+    (0 <= i) && (i < (R[Net#g] + C[Net#g])) ==> (SqnCh[Net#g][i] == i)
+  );
   assume C[Net#f] == 1;
-  assume C[Net#g] == R[Net#e];
+  assert {:msg "  52.15: "} C[Net#f] == 1;
+  assume (R[Net#g] + C[Net#g]) == R[Net#e];
+  assert {:msg "  53.15: "} (R[Net#g] + C[Net#g]) == R[Net#e];
   assume R[Net#e] == M[Net#f][R[Net#f]];
+  assert {:msg "  54.15: "} R[Net#e] == M[Net#f][R[Net#f]];
   assume (forall i: int :: 
     (0 <= i) && (i < (R[Net#g] + C[Net#g])) ==> (SqnCh[Net#g][i] == i)
   );
-  assume (0 < R[Net#d]) && (0 < R[Net#e]) ==> (M[Net#d][R[Net#d] - 1] <= M[Net#e][R[Net#e] - 1]);
+  assert {:msg "  55.16: "} (forall i: int :: 
+    (0 <= i) && (i < (R[Net#g] + C[Net#g])) ==> (SqnCh[Net#g][i] == i)
+  );
+  if ((0 < R[Net#d]) && (0 < R[Net#e])) {
+    assume M[Net#d][R[Net#d] - 1] <= M[Net#e][R[Net#e] - 1];
+    assert {:msg "  57.42: "} M[Net#d][R[Net#d] - 1] <= M[Net#e][R[Net#e] - 1];
+  }
   assume (forall i: int :: 
+    (0 <= i) && (i < R[Net#e]) ==> (M[Net#g][i] == M[Net#e][i])
+  );
+  assert {:msg "  58.16: "} (forall i: int :: 
     (0 <= i) && (i < R[Net#e]) ==> (M[Net#g][i] == M[Net#e][i])
   );
   assume true;
@@ -604,71 +834,57 @@ procedure Net#anon$3#Rep#anon$0#10()
   SqnCh[Net#e][R[Net#e] + C[Net#e]] := SqnAct[Net#sec];
   C[Net#e] := C[Net#e] + 1;
   SqnAct[Net#sec] := SqnAct[Net#sec] + 1;
-  assume 0 <= R[Net#a];
-  assume 0 <= C[Net#a];
-  assume (R[Net#a] + C[Net#a]) <= L[Net#a];
-  assume 0 <= R[Net#b];
-  assume 0 <= C[Net#b];
-  assume 0 <= R[Net#c];
-  assume 0 <= C[Net#c];
-  assume 0 <= R[Net#d];
-  assume 0 <= C[Net#d];
-  assume 0 <= R[Net#e];
-  assume 0 <= C[Net#e];
-  assume 0 <= R[Net#f];
-  assume 0 <= C[Net#f];
-  assume 0 <= R[Net#g];
-  assume 0 <= C[Net#g];
-  assume R[Net#g] == 0;
-  assert {:msg "  Action at 3.3 ('anon$0') for actor instance 'sec' might not preserve the channel invariant (#139)"} R[Net#a] == (R[Net#b] + C[Net#b]);
-  assert {:msg "  Action at 3.3 ('anon$0') for actor instance 'sec' might not preserve the channel invariant (#140)"} R[Net#a] == (R[Net#c] + C[Net#c]);
-  assert {:msg "  Action at 3.3 ('anon$0') for actor instance 'sec' might not preserve the channel invariant (#141)"} R[Net#b] == (R[Net#d] + C[Net#d]);
-  assert {:msg "  Action at 3.3 ('anon$0') for actor instance 'sec' might not preserve the channel invariant (#142)"} R[Net#c] == (R[Net#e] + C[Net#e]);
-  assert {:msg "  Action at 3.3 ('anon$0') for actor instance 'sec' might not preserve the channel invariant (#143)"} (forall idx$: int :: 
+  assert {:msg "  Action at 3.3 ('anon$0') for actor instance 'sec' might not preserve the channel invariant (#75)"} R[Net#a] == (R[Net#b] + C[Net#b]);
+  assert {:msg "  Action at 3.3 ('anon$0') for actor instance 'sec' might not preserve the channel invariant (#76)"} R[Net#a] == (R[Net#c] + C[Net#c]);
+  assert {:msg "  Action at 3.3 ('anon$0') for actor instance 'sec' might not preserve the channel invariant (#77)"} R[Net#b] == (R[Net#d] + C[Net#d]);
+  assert {:msg "  Action at 3.3 ('anon$0') for actor instance 'sec' might not preserve the channel invariant (#78)"} R[Net#c] == (R[Net#e] + C[Net#e]);
+  assert {:msg "  Action at 3.3 ('anon$0') for actor instance 'sec' might not preserve the channel invariant (#79)"} (forall idx$: int :: 
     (0 <= idx$) && (idx$ < (R[Net#b] + C[Net#b])) ==> (M[Net#b][idx$] == M[Net#a][idx$])
   );
-  assert {:msg "  Action at 3.3 ('anon$0') for actor instance 'sec' might not preserve the channel invariant (#144)"} (forall idx$: int :: 
+  assert {:msg "  Action at 3.3 ('anon$0') for actor instance 'sec' might not preserve the channel invariant (#80)"} (forall idx$: int :: 
     (0 <= idx$) && (idx$ < (R[Net#c] + C[Net#c])) ==> (M[Net#c][idx$] == M[Net#a][idx$])
   );
-  assert {:msg "  Action at 3.3 ('anon$0') for actor instance 'sec' might not preserve the channel invariant (#145)"} (forall idx$: int :: 
+  assert {:msg "  Action at 3.3 ('anon$0') for actor instance 'sec' might not preserve the channel invariant (#81)"} (forall idx$: int :: 
     (0 <= idx$) && (idx$ < (R[Net#d] + C[Net#d])) ==> (M[Net#d][idx$] == M[Net#b][idx$])
   );
-  assert {:msg "  Action at 3.3 ('anon$0') for actor instance 'sec' might not preserve the channel invariant (#146)"} (forall idx$: int :: 
+  assert {:msg "  Action at 3.3 ('anon$0') for actor instance 'sec' might not preserve the channel invariant (#82)"} (forall idx$: int :: 
     (0 <= idx$) && (idx$ < (R[Net#e] + C[Net#e])) ==> (M[Net#e][idx$] == M[Net#c][idx$])
   );
-  assert {:msg "  Action at 3.3 ('anon$0') for actor instance 'sec' might not preserve the channel invariant (#147)"} (forall idx$: int :: 
+  assert {:msg "  Action at 3.3 ('anon$0') for actor instance 'sec' might not preserve the channel invariant (#83)"} (forall idx$: int :: 
     (0 <= idx$) && (idx$ < (R[Net#a] + C[Net#a])) ==> (SqnCh[Net#a][idx$] == idx$)
   );
-  assert {:msg "  40.3: Action at 3.3 ('anon$0') for actor instance 'sec' might not preserve the channel invariant (#148)"} SqnAct[Net#spl] == R[Net#a];
-  assert {:msg "  41.3: Action at 3.3 ('anon$0') for actor instance 'sec' might not preserve the channel invariant (#149)"} SqnAct[Net#pri] == R[Net#b];
-  assert {:msg "  42.3: Action at 3.3 ('anon$0') for actor instance 'sec' might not preserve the channel invariant (#150)"} SqnAct[Net#sec] == R[Net#c];
-  assert {:msg "  43.3: Action at 3.3 ('anon$0') for actor instance 'sec' might not preserve the channel invariant (#151)"} SqnAct[Net#adj] == R[Net#e];
-  assert {:msg "  45.3: Action at 3.3 ('anon$0') for actor instance 'sec' might not preserve the channel invariant (#152)"} (forall i: int :: 
+  assert {:msg "  40.15: Action at 3.3 ('anon$0') for actor instance 'sec' might not preserve the channel invariant (#84)"} SqnAct[Net#spl] == R[Net#a];
+  assert {:msg "  41.15: Action at 3.3 ('anon$0') for actor instance 'sec' might not preserve the channel invariant (#85)"} SqnAct[Net#pri] == R[Net#b];
+  assert {:msg "  42.15: Action at 3.3 ('anon$0') for actor instance 'sec' might not preserve the channel invariant (#86)"} SqnAct[Net#sec] == R[Net#c];
+  assert {:msg "  43.15: Action at 3.3 ('anon$0') for actor instance 'sec' might not preserve the channel invariant (#87)"} SqnAct[Net#adj] == R[Net#e];
+  assert {:msg "  45.16: Action at 3.3 ('anon$0') for actor instance 'sec' might not preserve the channel invariant (#88)"} (forall i: int :: 
     (0 <= i) && (i < (R[Net#a] + C[Net#a])) ==> (SqnCh[Net#a][i] == i)
   );
-  assert {:msg "  46.3: Action at 3.3 ('anon$0') for actor instance 'sec' might not preserve the channel invariant (#153)"} (forall i: int :: 
+  assert {:msg "  46.16: Action at 3.3 ('anon$0') for actor instance 'sec' might not preserve the channel invariant (#89)"} (forall i: int :: 
     (0 <= i) && (i < (R[Net#b] + C[Net#b])) ==> (SqnCh[Net#b][i] == i)
   );
-  assert {:msg "  47.3: Action at 3.3 ('anon$0') for actor instance 'sec' might not preserve the channel invariant (#154)"} (forall i: int :: 
+  assert {:msg "  47.16: Action at 3.3 ('anon$0') for actor instance 'sec' might not preserve the channel invariant (#90)"} (forall i: int :: 
     (0 <= i) && (i < (R[Net#c] + C[Net#c])) ==> (SqnCh[Net#c][i] == i)
   );
-  assert {:msg "  48.3: Action at 3.3 ('anon$0') for actor instance 'sec' might not preserve the channel invariant (#155)"} (forall i: int :: 
+  assert {:msg "  48.16: Action at 3.3 ('anon$0') for actor instance 'sec' might not preserve the channel invariant (#91)"} (forall i: int :: 
     (0 <= i) && (i < (R[Net#d] + C[Net#d])) ==> (SqnCh[Net#d][i] == i)
   );
-  assert {:msg "  49.3: Action at 3.3 ('anon$0') for actor instance 'sec' might not preserve the channel invariant (#156)"} (forall i: int :: 
+  assert {:msg "  49.16: Action at 3.3 ('anon$0') for actor instance 'sec' might not preserve the channel invariant (#92)"} (forall i: int :: 
     (0 <= i) && (i < (R[Net#e] + C[Net#e])) ==> (SqnCh[Net#e][i] == i)
   );
-  assert {:msg "  50.3: Action at 3.3 ('anon$0') for actor instance 'sec' might not preserve the channel invariant (#157)"} (forall i: int :: 
+  assert {:msg "  50.16: Action at 3.3 ('anon$0') for actor instance 'sec' might not preserve the channel invariant (#93)"} (forall i: int :: 
     (0 <= i) && (i < (R[Net#g] + C[Net#g])) ==> (SqnCh[Net#g][i] == i)
   );
-  assert {:msg "  52.3: Action at 3.3 ('anon$0') for actor instance 'sec' might not preserve the channel invariant (#158)"} C[Net#f] == 1;
-  assert {:msg "  53.3: Action at 3.3 ('anon$0') for actor instance 'sec' might not preserve the channel invariant (#159)"} C[Net#g] == R[Net#e];
-  assert {:msg "  54.3: Action at 3.3 ('anon$0') for actor instance 'sec' might not preserve the channel invariant (#160)"} R[Net#e] == M[Net#f][R[Net#f]];
-  assert {:msg "  55.3: Action at 3.3 ('anon$0') for actor instance 'sec' might not preserve the channel invariant (#161)"} (forall i: int :: 
+  assert {:msg "  52.15: Action at 3.3 ('anon$0') for actor instance 'sec' might not preserve the channel invariant (#94)"} C[Net#f] == 1;
+  assert {:msg "  53.15: Action at 3.3 ('anon$0') for actor instance 'sec' might not preserve the channel invariant (#95)"} (R[Net#g] + C[Net#g]) == R[Net#e];
+  assert {:msg "  54.15: Action at 3.3 ('anon$0') for actor instance 'sec' might not preserve the channel invariant (#96)"} R[Net#e] == M[Net#f][R[Net#f]];
+  assert {:msg "  55.16: Action at 3.3 ('anon$0') for actor instance 'sec' might not preserve the channel invariant (#97)"} (forall i: int :: 
     (0 <= i) && (i < (R[Net#g] + C[Net#g])) ==> (SqnCh[Net#g][i] == i)
   );
-  assert {:msg "  59.3: Action at 3.3 ('anon$0') for actor instance 'sec' might not preserve the channel invariant (#162)"} (0 < R[Net#d]) && (0 < R[Net#e]) ==> (M[Net#d][R[Net#d] - 1] <= M[Net#e][R[Net#e] - 1]);
-  assert {:msg "  60.3: Action at 3.3 ('anon$0') for actor instance 'sec' might not preserve the channel invariant (#163)"} (forall i: int :: 
+  if ((0 < R[Net#d]) && (0 < R[Net#e])) {
+    assert {:msg "  57.42: Action at 3.3 ('anon$0') for actor instance 'sec' might not preserve the channel invariant (#98)"} M[Net#d][R[Net#d] - 1] <= M[Net#e][R[Net#e] - 1];
+  }
+  assert {:msg "  58.16: Action at 3.3 ('anon$0') for actor instance 'sec' might not preserve the channel invariant (#99)"} (forall i: int :: 
     (0 <= i) && (i < R[Net#e]) ==> (M[Net#g][i] == M[Net#e][i])
   );
 }
@@ -696,54 +912,107 @@ procedure Net#anon$3#Adjudicator#readoff#11()
   assume 0 <= C[Net#g];
   assume R[Net#g] == 0;
   assume R[Net#a] == (R[Net#b] + C[Net#b]);
+  assert {:msg "  "} R[Net#a] == (R[Net#b] + C[Net#b]);
   assume R[Net#a] == (R[Net#c] + C[Net#c]);
+  assert {:msg "  "} R[Net#a] == (R[Net#c] + C[Net#c]);
   assume R[Net#b] == (R[Net#d] + C[Net#d]);
+  assert {:msg "  "} R[Net#b] == (R[Net#d] + C[Net#d]);
   assume R[Net#c] == (R[Net#e] + C[Net#e]);
+  assert {:msg "  "} R[Net#c] == (R[Net#e] + C[Net#e]);
   assume (forall idx$: int :: 
+    (0 <= idx$) && (idx$ < (R[Net#b] + C[Net#b])) ==> (M[Net#b][idx$] == M[Net#a][idx$])
+  );
+  assert {:msg "  "} (forall idx$: int :: 
     (0 <= idx$) && (idx$ < (R[Net#b] + C[Net#b])) ==> (M[Net#b][idx$] == M[Net#a][idx$])
   );
   assume (forall idx$: int :: 
     (0 <= idx$) && (idx$ < (R[Net#c] + C[Net#c])) ==> (M[Net#c][idx$] == M[Net#a][idx$])
   );
+  assert {:msg "  "} (forall idx$: int :: 
+    (0 <= idx$) && (idx$ < (R[Net#c] + C[Net#c])) ==> (M[Net#c][idx$] == M[Net#a][idx$])
+  );
   assume (forall idx$: int :: 
+    (0 <= idx$) && (idx$ < (R[Net#d] + C[Net#d])) ==> (M[Net#d][idx$] == M[Net#b][idx$])
+  );
+  assert {:msg "  "} (forall idx$: int :: 
     (0 <= idx$) && (idx$ < (R[Net#d] + C[Net#d])) ==> (M[Net#d][idx$] == M[Net#b][idx$])
   );
   assume (forall idx$: int :: 
     (0 <= idx$) && (idx$ < (R[Net#e] + C[Net#e])) ==> (M[Net#e][idx$] == M[Net#c][idx$])
   );
+  assert {:msg "  "} (forall idx$: int :: 
+    (0 <= idx$) && (idx$ < (R[Net#e] + C[Net#e])) ==> (M[Net#e][idx$] == M[Net#c][idx$])
+  );
   assume (forall idx$: int :: 
     (0 <= idx$) && (idx$ < (R[Net#a] + C[Net#a])) ==> (SqnCh[Net#a][idx$] == idx$)
   );
+  assert {:msg "  "} (forall idx$: int :: 
+    (0 <= idx$) && (idx$ < (R[Net#a] + C[Net#a])) ==> (SqnCh[Net#a][idx$] == idx$)
+  );
   assume SqnAct[Net#spl] == R[Net#a];
+  assert {:msg "  40.15: "} SqnAct[Net#spl] == R[Net#a];
   assume SqnAct[Net#pri] == R[Net#b];
+  assert {:msg "  41.15: "} SqnAct[Net#pri] == R[Net#b];
   assume SqnAct[Net#sec] == R[Net#c];
+  assert {:msg "  42.15: "} SqnAct[Net#sec] == R[Net#c];
   assume SqnAct[Net#adj] == R[Net#e];
+  assert {:msg "  43.15: "} SqnAct[Net#adj] == R[Net#e];
   assume (forall i: int :: 
+    (0 <= i) && (i < (R[Net#a] + C[Net#a])) ==> (SqnCh[Net#a][i] == i)
+  );
+  assert {:msg "  45.16: "} (forall i: int :: 
     (0 <= i) && (i < (R[Net#a] + C[Net#a])) ==> (SqnCh[Net#a][i] == i)
   );
   assume (forall i: int :: 
     (0 <= i) && (i < (R[Net#b] + C[Net#b])) ==> (SqnCh[Net#b][i] == i)
   );
+  assert {:msg "  46.16: "} (forall i: int :: 
+    (0 <= i) && (i < (R[Net#b] + C[Net#b])) ==> (SqnCh[Net#b][i] == i)
+  );
   assume (forall i: int :: 
+    (0 <= i) && (i < (R[Net#c] + C[Net#c])) ==> (SqnCh[Net#c][i] == i)
+  );
+  assert {:msg "  47.16: "} (forall i: int :: 
     (0 <= i) && (i < (R[Net#c] + C[Net#c])) ==> (SqnCh[Net#c][i] == i)
   );
   assume (forall i: int :: 
     (0 <= i) && (i < (R[Net#d] + C[Net#d])) ==> (SqnCh[Net#d][i] == i)
   );
+  assert {:msg "  48.16: "} (forall i: int :: 
+    (0 <= i) && (i < (R[Net#d] + C[Net#d])) ==> (SqnCh[Net#d][i] == i)
+  );
   assume (forall i: int :: 
+    (0 <= i) && (i < (R[Net#e] + C[Net#e])) ==> (SqnCh[Net#e][i] == i)
+  );
+  assert {:msg "  49.16: "} (forall i: int :: 
     (0 <= i) && (i < (R[Net#e] + C[Net#e])) ==> (SqnCh[Net#e][i] == i)
   );
   assume (forall i: int :: 
     (0 <= i) && (i < (R[Net#g] + C[Net#g])) ==> (SqnCh[Net#g][i] == i)
   );
+  assert {:msg "  50.16: "} (forall i: int :: 
+    (0 <= i) && (i < (R[Net#g] + C[Net#g])) ==> (SqnCh[Net#g][i] == i)
+  );
   assume C[Net#f] == 1;
-  assume C[Net#g] == R[Net#e];
+  assert {:msg "  52.15: "} C[Net#f] == 1;
+  assume (R[Net#g] + C[Net#g]) == R[Net#e];
+  assert {:msg "  53.15: "} (R[Net#g] + C[Net#g]) == R[Net#e];
   assume R[Net#e] == M[Net#f][R[Net#f]];
+  assert {:msg "  54.15: "} R[Net#e] == M[Net#f][R[Net#f]];
   assume (forall i: int :: 
     (0 <= i) && (i < (R[Net#g] + C[Net#g])) ==> (SqnCh[Net#g][i] == i)
   );
-  assume (0 < R[Net#d]) && (0 < R[Net#e]) ==> (M[Net#d][R[Net#d] - 1] <= M[Net#e][R[Net#e] - 1]);
+  assert {:msg "  55.16: "} (forall i: int :: 
+    (0 <= i) && (i < (R[Net#g] + C[Net#g])) ==> (SqnCh[Net#g][i] == i)
+  );
+  if ((0 < R[Net#d]) && (0 < R[Net#e])) {
+    assume M[Net#d][R[Net#d] - 1] <= M[Net#e][R[Net#e] - 1];
+    assert {:msg "  57.42: "} M[Net#d][R[Net#d] - 1] <= M[Net#e][R[Net#e] - 1];
+  }
   assume (forall i: int :: 
+    (0 <= i) && (i < R[Net#e]) ==> (M[Net#g][i] == M[Net#e][i])
+  );
+  assert {:msg "  58.16: "} (forall i: int :: 
     (0 <= i) && (i < R[Net#e]) ==> (M[Net#g][i] == M[Net#e][i])
   );
   assume SqnCh[Net#d][R[Net#d] - 0] < M[Net#f][R[Net#f] - 0];
@@ -758,71 +1027,57 @@ procedure Net#anon$3#Adjudicator#readoff#11()
   M[Net#f][R[Net#f] + C[Net#f]] := c_in#c;
   SqnCh[Net#f][R[Net#f] + C[Net#f]] := SqnAct[Net#adj];
   C[Net#f] := C[Net#f] + 1;
-  assume 0 <= R[Net#a];
-  assume 0 <= C[Net#a];
-  assume (R[Net#a] + C[Net#a]) <= L[Net#a];
-  assume 0 <= R[Net#b];
-  assume 0 <= C[Net#b];
-  assume 0 <= R[Net#c];
-  assume 0 <= C[Net#c];
-  assume 0 <= R[Net#d];
-  assume 0 <= C[Net#d];
-  assume 0 <= R[Net#e];
-  assume 0 <= C[Net#e];
-  assume 0 <= R[Net#f];
-  assume 0 <= C[Net#f];
-  assume 0 <= R[Net#g];
-  assume 0 <= C[Net#g];
-  assume R[Net#g] == 0;
-  assert {:msg "  Action at 20.3 ('readoff') for actor instance 'adj' might not preserve the channel invariant (#180)"} R[Net#a] == (R[Net#b] + C[Net#b]);
-  assert {:msg "  Action at 20.3 ('readoff') for actor instance 'adj' might not preserve the channel invariant (#181)"} R[Net#a] == (R[Net#c] + C[Net#c]);
-  assert {:msg "  Action at 20.3 ('readoff') for actor instance 'adj' might not preserve the channel invariant (#182)"} R[Net#b] == (R[Net#d] + C[Net#d]);
-  assert {:msg "  Action at 20.3 ('readoff') for actor instance 'adj' might not preserve the channel invariant (#183)"} R[Net#c] == (R[Net#e] + C[Net#e]);
-  assert {:msg "  Action at 20.3 ('readoff') for actor instance 'adj' might not preserve the channel invariant (#184)"} (forall idx$: int :: 
+  assert {:msg "  Action at 20.3 ('readoff') for actor instance 'adj' might not preserve the channel invariant (#100)"} R[Net#a] == (R[Net#b] + C[Net#b]);
+  assert {:msg "  Action at 20.3 ('readoff') for actor instance 'adj' might not preserve the channel invariant (#101)"} R[Net#a] == (R[Net#c] + C[Net#c]);
+  assert {:msg "  Action at 20.3 ('readoff') for actor instance 'adj' might not preserve the channel invariant (#102)"} R[Net#b] == (R[Net#d] + C[Net#d]);
+  assert {:msg "  Action at 20.3 ('readoff') for actor instance 'adj' might not preserve the channel invariant (#103)"} R[Net#c] == (R[Net#e] + C[Net#e]);
+  assert {:msg "  Action at 20.3 ('readoff') for actor instance 'adj' might not preserve the channel invariant (#104)"} (forall idx$: int :: 
     (0 <= idx$) && (idx$ < (R[Net#b] + C[Net#b])) ==> (M[Net#b][idx$] == M[Net#a][idx$])
   );
-  assert {:msg "  Action at 20.3 ('readoff') for actor instance 'adj' might not preserve the channel invariant (#185)"} (forall idx$: int :: 
+  assert {:msg "  Action at 20.3 ('readoff') for actor instance 'adj' might not preserve the channel invariant (#105)"} (forall idx$: int :: 
     (0 <= idx$) && (idx$ < (R[Net#c] + C[Net#c])) ==> (M[Net#c][idx$] == M[Net#a][idx$])
   );
-  assert {:msg "  Action at 20.3 ('readoff') for actor instance 'adj' might not preserve the channel invariant (#186)"} (forall idx$: int :: 
+  assert {:msg "  Action at 20.3 ('readoff') for actor instance 'adj' might not preserve the channel invariant (#106)"} (forall idx$: int :: 
     (0 <= idx$) && (idx$ < (R[Net#d] + C[Net#d])) ==> (M[Net#d][idx$] == M[Net#b][idx$])
   );
-  assert {:msg "  Action at 20.3 ('readoff') for actor instance 'adj' might not preserve the channel invariant (#187)"} (forall idx$: int :: 
+  assert {:msg "  Action at 20.3 ('readoff') for actor instance 'adj' might not preserve the channel invariant (#107)"} (forall idx$: int :: 
     (0 <= idx$) && (idx$ < (R[Net#e] + C[Net#e])) ==> (M[Net#e][idx$] == M[Net#c][idx$])
   );
-  assert {:msg "  Action at 20.3 ('readoff') for actor instance 'adj' might not preserve the channel invariant (#188)"} (forall idx$: int :: 
+  assert {:msg "  Action at 20.3 ('readoff') for actor instance 'adj' might not preserve the channel invariant (#108)"} (forall idx$: int :: 
     (0 <= idx$) && (idx$ < (R[Net#a] + C[Net#a])) ==> (SqnCh[Net#a][idx$] == idx$)
   );
-  assert {:msg "  40.3: Action at 20.3 ('readoff') for actor instance 'adj' might not preserve the channel invariant (#189)"} SqnAct[Net#spl] == R[Net#a];
-  assert {:msg "  41.3: Action at 20.3 ('readoff') for actor instance 'adj' might not preserve the channel invariant (#190)"} SqnAct[Net#pri] == R[Net#b];
-  assert {:msg "  42.3: Action at 20.3 ('readoff') for actor instance 'adj' might not preserve the channel invariant (#191)"} SqnAct[Net#sec] == R[Net#c];
-  assert {:msg "  43.3: Action at 20.3 ('readoff') for actor instance 'adj' might not preserve the channel invariant (#192)"} SqnAct[Net#adj] == R[Net#e];
-  assert {:msg "  45.3: Action at 20.3 ('readoff') for actor instance 'adj' might not preserve the channel invariant (#193)"} (forall i: int :: 
+  assert {:msg "  40.15: Action at 20.3 ('readoff') for actor instance 'adj' might not preserve the channel invariant (#109)"} SqnAct[Net#spl] == R[Net#a];
+  assert {:msg "  41.15: Action at 20.3 ('readoff') for actor instance 'adj' might not preserve the channel invariant (#110)"} SqnAct[Net#pri] == R[Net#b];
+  assert {:msg "  42.15: Action at 20.3 ('readoff') for actor instance 'adj' might not preserve the channel invariant (#111)"} SqnAct[Net#sec] == R[Net#c];
+  assert {:msg "  43.15: Action at 20.3 ('readoff') for actor instance 'adj' might not preserve the channel invariant (#112)"} SqnAct[Net#adj] == R[Net#e];
+  assert {:msg "  45.16: Action at 20.3 ('readoff') for actor instance 'adj' might not preserve the channel invariant (#113)"} (forall i: int :: 
     (0 <= i) && (i < (R[Net#a] + C[Net#a])) ==> (SqnCh[Net#a][i] == i)
   );
-  assert {:msg "  46.3: Action at 20.3 ('readoff') for actor instance 'adj' might not preserve the channel invariant (#194)"} (forall i: int :: 
+  assert {:msg "  46.16: Action at 20.3 ('readoff') for actor instance 'adj' might not preserve the channel invariant (#114)"} (forall i: int :: 
     (0 <= i) && (i < (R[Net#b] + C[Net#b])) ==> (SqnCh[Net#b][i] == i)
   );
-  assert {:msg "  47.3: Action at 20.3 ('readoff') for actor instance 'adj' might not preserve the channel invariant (#195)"} (forall i: int :: 
+  assert {:msg "  47.16: Action at 20.3 ('readoff') for actor instance 'adj' might not preserve the channel invariant (#115)"} (forall i: int :: 
     (0 <= i) && (i < (R[Net#c] + C[Net#c])) ==> (SqnCh[Net#c][i] == i)
   );
-  assert {:msg "  48.3: Action at 20.3 ('readoff') for actor instance 'adj' might not preserve the channel invariant (#196)"} (forall i: int :: 
+  assert {:msg "  48.16: Action at 20.3 ('readoff') for actor instance 'adj' might not preserve the channel invariant (#116)"} (forall i: int :: 
     (0 <= i) && (i < (R[Net#d] + C[Net#d])) ==> (SqnCh[Net#d][i] == i)
   );
-  assert {:msg "  49.3: Action at 20.3 ('readoff') for actor instance 'adj' might not preserve the channel invariant (#197)"} (forall i: int :: 
+  assert {:msg "  49.16: Action at 20.3 ('readoff') for actor instance 'adj' might not preserve the channel invariant (#117)"} (forall i: int :: 
     (0 <= i) && (i < (R[Net#e] + C[Net#e])) ==> (SqnCh[Net#e][i] == i)
   );
-  assert {:msg "  50.3: Action at 20.3 ('readoff') for actor instance 'adj' might not preserve the channel invariant (#198)"} (forall i: int :: 
+  assert {:msg "  50.16: Action at 20.3 ('readoff') for actor instance 'adj' might not preserve the channel invariant (#118)"} (forall i: int :: 
     (0 <= i) && (i < (R[Net#g] + C[Net#g])) ==> (SqnCh[Net#g][i] == i)
   );
-  assert {:msg "  52.3: Action at 20.3 ('readoff') for actor instance 'adj' might not preserve the channel invariant (#199)"} C[Net#f] == 1;
-  assert {:msg "  53.3: Action at 20.3 ('readoff') for actor instance 'adj' might not preserve the channel invariant (#200)"} C[Net#g] == R[Net#e];
-  assert {:msg "  54.3: Action at 20.3 ('readoff') for actor instance 'adj' might not preserve the channel invariant (#201)"} R[Net#e] == M[Net#f][R[Net#f]];
-  assert {:msg "  55.3: Action at 20.3 ('readoff') for actor instance 'adj' might not preserve the channel invariant (#202)"} (forall i: int :: 
+  assert {:msg "  52.15: Action at 20.3 ('readoff') for actor instance 'adj' might not preserve the channel invariant (#119)"} C[Net#f] == 1;
+  assert {:msg "  53.15: Action at 20.3 ('readoff') for actor instance 'adj' might not preserve the channel invariant (#120)"} (R[Net#g] + C[Net#g]) == R[Net#e];
+  assert {:msg "  54.15: Action at 20.3 ('readoff') for actor instance 'adj' might not preserve the channel invariant (#121)"} R[Net#e] == M[Net#f][R[Net#f]];
+  assert {:msg "  55.16: Action at 20.3 ('readoff') for actor instance 'adj' might not preserve the channel invariant (#122)"} (forall i: int :: 
     (0 <= i) && (i < (R[Net#g] + C[Net#g])) ==> (SqnCh[Net#g][i] == i)
   );
-  assert {:msg "  59.3: Action at 20.3 ('readoff') for actor instance 'adj' might not preserve the channel invariant (#203)"} (0 < R[Net#d]) && (0 < R[Net#e]) ==> (M[Net#d][R[Net#d] - 1] <= M[Net#e][R[Net#e] - 1]);
-  assert {:msg "  60.3: Action at 20.3 ('readoff') for actor instance 'adj' might not preserve the channel invariant (#204)"} (forall i: int :: 
+  if ((0 < R[Net#d]) && (0 < R[Net#e])) {
+    assert {:msg "  57.42: Action at 20.3 ('readoff') for actor instance 'adj' might not preserve the channel invariant (#123)"} M[Net#d][R[Net#d] - 1] <= M[Net#e][R[Net#e] - 1];
+  }
+  assert {:msg "  58.16: Action at 20.3 ('readoff') for actor instance 'adj' might not preserve the channel invariant (#124)"} (forall i: int :: 
     (0 <= i) && (i < R[Net#e]) ==> (M[Net#g][i] == M[Net#e][i])
   );
 }
@@ -851,54 +1106,107 @@ procedure Net#anon$3#Adjudicator#normal#12()
   assume 0 <= C[Net#g];
   assume R[Net#g] == 0;
   assume R[Net#a] == (R[Net#b] + C[Net#b]);
+  assert {:msg "  "} R[Net#a] == (R[Net#b] + C[Net#b]);
   assume R[Net#a] == (R[Net#c] + C[Net#c]);
+  assert {:msg "  "} R[Net#a] == (R[Net#c] + C[Net#c]);
   assume R[Net#b] == (R[Net#d] + C[Net#d]);
+  assert {:msg "  "} R[Net#b] == (R[Net#d] + C[Net#d]);
   assume R[Net#c] == (R[Net#e] + C[Net#e]);
+  assert {:msg "  "} R[Net#c] == (R[Net#e] + C[Net#e]);
   assume (forall idx$: int :: 
+    (0 <= idx$) && (idx$ < (R[Net#b] + C[Net#b])) ==> (M[Net#b][idx$] == M[Net#a][idx$])
+  );
+  assert {:msg "  "} (forall idx$: int :: 
     (0 <= idx$) && (idx$ < (R[Net#b] + C[Net#b])) ==> (M[Net#b][idx$] == M[Net#a][idx$])
   );
   assume (forall idx$: int :: 
     (0 <= idx$) && (idx$ < (R[Net#c] + C[Net#c])) ==> (M[Net#c][idx$] == M[Net#a][idx$])
   );
+  assert {:msg "  "} (forall idx$: int :: 
+    (0 <= idx$) && (idx$ < (R[Net#c] + C[Net#c])) ==> (M[Net#c][idx$] == M[Net#a][idx$])
+  );
   assume (forall idx$: int :: 
+    (0 <= idx$) && (idx$ < (R[Net#d] + C[Net#d])) ==> (M[Net#d][idx$] == M[Net#b][idx$])
+  );
+  assert {:msg "  "} (forall idx$: int :: 
     (0 <= idx$) && (idx$ < (R[Net#d] + C[Net#d])) ==> (M[Net#d][idx$] == M[Net#b][idx$])
   );
   assume (forall idx$: int :: 
     (0 <= idx$) && (idx$ < (R[Net#e] + C[Net#e])) ==> (M[Net#e][idx$] == M[Net#c][idx$])
   );
+  assert {:msg "  "} (forall idx$: int :: 
+    (0 <= idx$) && (idx$ < (R[Net#e] + C[Net#e])) ==> (M[Net#e][idx$] == M[Net#c][idx$])
+  );
   assume (forall idx$: int :: 
     (0 <= idx$) && (idx$ < (R[Net#a] + C[Net#a])) ==> (SqnCh[Net#a][idx$] == idx$)
   );
+  assert {:msg "  "} (forall idx$: int :: 
+    (0 <= idx$) && (idx$ < (R[Net#a] + C[Net#a])) ==> (SqnCh[Net#a][idx$] == idx$)
+  );
   assume SqnAct[Net#spl] == R[Net#a];
+  assert {:msg "  40.15: "} SqnAct[Net#spl] == R[Net#a];
   assume SqnAct[Net#pri] == R[Net#b];
+  assert {:msg "  41.15: "} SqnAct[Net#pri] == R[Net#b];
   assume SqnAct[Net#sec] == R[Net#c];
+  assert {:msg "  42.15: "} SqnAct[Net#sec] == R[Net#c];
   assume SqnAct[Net#adj] == R[Net#e];
+  assert {:msg "  43.15: "} SqnAct[Net#adj] == R[Net#e];
   assume (forall i: int :: 
+    (0 <= i) && (i < (R[Net#a] + C[Net#a])) ==> (SqnCh[Net#a][i] == i)
+  );
+  assert {:msg "  45.16: "} (forall i: int :: 
     (0 <= i) && (i < (R[Net#a] + C[Net#a])) ==> (SqnCh[Net#a][i] == i)
   );
   assume (forall i: int :: 
     (0 <= i) && (i < (R[Net#b] + C[Net#b])) ==> (SqnCh[Net#b][i] == i)
   );
+  assert {:msg "  46.16: "} (forall i: int :: 
+    (0 <= i) && (i < (R[Net#b] + C[Net#b])) ==> (SqnCh[Net#b][i] == i)
+  );
   assume (forall i: int :: 
+    (0 <= i) && (i < (R[Net#c] + C[Net#c])) ==> (SqnCh[Net#c][i] == i)
+  );
+  assert {:msg "  47.16: "} (forall i: int :: 
     (0 <= i) && (i < (R[Net#c] + C[Net#c])) ==> (SqnCh[Net#c][i] == i)
   );
   assume (forall i: int :: 
     (0 <= i) && (i < (R[Net#d] + C[Net#d])) ==> (SqnCh[Net#d][i] == i)
   );
+  assert {:msg "  48.16: "} (forall i: int :: 
+    (0 <= i) && (i < (R[Net#d] + C[Net#d])) ==> (SqnCh[Net#d][i] == i)
+  );
   assume (forall i: int :: 
+    (0 <= i) && (i < (R[Net#e] + C[Net#e])) ==> (SqnCh[Net#e][i] == i)
+  );
+  assert {:msg "  49.16: "} (forall i: int :: 
     (0 <= i) && (i < (R[Net#e] + C[Net#e])) ==> (SqnCh[Net#e][i] == i)
   );
   assume (forall i: int :: 
     (0 <= i) && (i < (R[Net#g] + C[Net#g])) ==> (SqnCh[Net#g][i] == i)
   );
+  assert {:msg "  50.16: "} (forall i: int :: 
+    (0 <= i) && (i < (R[Net#g] + C[Net#g])) ==> (SqnCh[Net#g][i] == i)
+  );
   assume C[Net#f] == 1;
-  assume C[Net#g] == R[Net#e];
+  assert {:msg "  52.15: "} C[Net#f] == 1;
+  assume (R[Net#g] + C[Net#g]) == R[Net#e];
+  assert {:msg "  53.15: "} (R[Net#g] + C[Net#g]) == R[Net#e];
   assume R[Net#e] == M[Net#f][R[Net#f]];
+  assert {:msg "  54.15: "} R[Net#e] == M[Net#f][R[Net#f]];
   assume (forall i: int :: 
     (0 <= i) && (i < (R[Net#g] + C[Net#g])) ==> (SqnCh[Net#g][i] == i)
   );
-  assume (0 < R[Net#d]) && (0 < R[Net#e]) ==> (M[Net#d][R[Net#d] - 1] <= M[Net#e][R[Net#e] - 1]);
+  assert {:msg "  55.16: "} (forall i: int :: 
+    (0 <= i) && (i < (R[Net#g] + C[Net#g])) ==> (SqnCh[Net#g][i] == i)
+  );
+  if ((0 < R[Net#d]) && (0 < R[Net#e])) {
+    assume M[Net#d][R[Net#d] - 1] <= M[Net#e][R[Net#e] - 1];
+    assert {:msg "  57.42: "} M[Net#d][R[Net#d] - 1] <= M[Net#e][R[Net#e] - 1];
+  }
   assume (forall i: int :: 
+    (0 <= i) && (i < R[Net#e]) ==> (M[Net#g][i] == M[Net#e][i])
+  );
+  assert {:msg "  58.16: "} (forall i: int :: 
     (0 <= i) && (i < R[Net#e]) ==> (M[Net#g][i] == M[Net#e][i])
   );
   assume (SqnCh[Net#d][R[Net#d] - 0] == SqnCh[Net#e][R[Net#e] - 0]) && (SqnCh[Net#d][R[Net#d] - 0] == M[Net#f][R[Net#f] - 0]);
@@ -920,71 +1228,57 @@ procedure Net#anon$3#Adjudicator#normal#12()
   SqnCh[Net#f][R[Net#f] + C[Net#f]] := SqnAct[Net#adj];
   C[Net#f] := C[Net#f] + 1;
   SqnAct[Net#adj] := SqnAct[Net#adj] + 1;
-  assume 0 <= R[Net#a];
-  assume 0 <= C[Net#a];
-  assume (R[Net#a] + C[Net#a]) <= L[Net#a];
-  assume 0 <= R[Net#b];
-  assume 0 <= C[Net#b];
-  assume 0 <= R[Net#c];
-  assume 0 <= C[Net#c];
-  assume 0 <= R[Net#d];
-  assume 0 <= C[Net#d];
-  assume 0 <= R[Net#e];
-  assume 0 <= C[Net#e];
-  assume 0 <= R[Net#f];
-  assume 0 <= C[Net#f];
-  assume 0 <= R[Net#g];
-  assume 0 <= C[Net#g];
-  assume R[Net#g] == 0;
-  assert {:msg "  Action at 14.3 ('normal') for actor instance 'adj' might not preserve the channel invariant (#221)"} R[Net#a] == (R[Net#b] + C[Net#b]);
-  assert {:msg "  Action at 14.3 ('normal') for actor instance 'adj' might not preserve the channel invariant (#222)"} R[Net#a] == (R[Net#c] + C[Net#c]);
-  assert {:msg "  Action at 14.3 ('normal') for actor instance 'adj' might not preserve the channel invariant (#223)"} R[Net#b] == (R[Net#d] + C[Net#d]);
-  assert {:msg "  Action at 14.3 ('normal') for actor instance 'adj' might not preserve the channel invariant (#224)"} R[Net#c] == (R[Net#e] + C[Net#e]);
-  assert {:msg "  Action at 14.3 ('normal') for actor instance 'adj' might not preserve the channel invariant (#225)"} (forall idx$: int :: 
+  assert {:msg "  Action at 14.3 ('normal') for actor instance 'adj' might not preserve the channel invariant (#125)"} R[Net#a] == (R[Net#b] + C[Net#b]);
+  assert {:msg "  Action at 14.3 ('normal') for actor instance 'adj' might not preserve the channel invariant (#126)"} R[Net#a] == (R[Net#c] + C[Net#c]);
+  assert {:msg "  Action at 14.3 ('normal') for actor instance 'adj' might not preserve the channel invariant (#127)"} R[Net#b] == (R[Net#d] + C[Net#d]);
+  assert {:msg "  Action at 14.3 ('normal') for actor instance 'adj' might not preserve the channel invariant (#128)"} R[Net#c] == (R[Net#e] + C[Net#e]);
+  assert {:msg "  Action at 14.3 ('normal') for actor instance 'adj' might not preserve the channel invariant (#129)"} (forall idx$: int :: 
     (0 <= idx$) && (idx$ < (R[Net#b] + C[Net#b])) ==> (M[Net#b][idx$] == M[Net#a][idx$])
   );
-  assert {:msg "  Action at 14.3 ('normal') for actor instance 'adj' might not preserve the channel invariant (#226)"} (forall idx$: int :: 
+  assert {:msg "  Action at 14.3 ('normal') for actor instance 'adj' might not preserve the channel invariant (#130)"} (forall idx$: int :: 
     (0 <= idx$) && (idx$ < (R[Net#c] + C[Net#c])) ==> (M[Net#c][idx$] == M[Net#a][idx$])
   );
-  assert {:msg "  Action at 14.3 ('normal') for actor instance 'adj' might not preserve the channel invariant (#227)"} (forall idx$: int :: 
+  assert {:msg "  Action at 14.3 ('normal') for actor instance 'adj' might not preserve the channel invariant (#131)"} (forall idx$: int :: 
     (0 <= idx$) && (idx$ < (R[Net#d] + C[Net#d])) ==> (M[Net#d][idx$] == M[Net#b][idx$])
   );
-  assert {:msg "  Action at 14.3 ('normal') for actor instance 'adj' might not preserve the channel invariant (#228)"} (forall idx$: int :: 
+  assert {:msg "  Action at 14.3 ('normal') for actor instance 'adj' might not preserve the channel invariant (#132)"} (forall idx$: int :: 
     (0 <= idx$) && (idx$ < (R[Net#e] + C[Net#e])) ==> (M[Net#e][idx$] == M[Net#c][idx$])
   );
-  assert {:msg "  Action at 14.3 ('normal') for actor instance 'adj' might not preserve the channel invariant (#229)"} (forall idx$: int :: 
+  assert {:msg "  Action at 14.3 ('normal') for actor instance 'adj' might not preserve the channel invariant (#133)"} (forall idx$: int :: 
     (0 <= idx$) && (idx$ < (R[Net#a] + C[Net#a])) ==> (SqnCh[Net#a][idx$] == idx$)
   );
-  assert {:msg "  40.3: Action at 14.3 ('normal') for actor instance 'adj' might not preserve the channel invariant (#230)"} SqnAct[Net#spl] == R[Net#a];
-  assert {:msg "  41.3: Action at 14.3 ('normal') for actor instance 'adj' might not preserve the channel invariant (#231)"} SqnAct[Net#pri] == R[Net#b];
-  assert {:msg "  42.3: Action at 14.3 ('normal') for actor instance 'adj' might not preserve the channel invariant (#232)"} SqnAct[Net#sec] == R[Net#c];
-  assert {:msg "  43.3: Action at 14.3 ('normal') for actor instance 'adj' might not preserve the channel invariant (#233)"} SqnAct[Net#adj] == R[Net#e];
-  assert {:msg "  45.3: Action at 14.3 ('normal') for actor instance 'adj' might not preserve the channel invariant (#234)"} (forall i: int :: 
+  assert {:msg "  40.15: Action at 14.3 ('normal') for actor instance 'adj' might not preserve the channel invariant (#134)"} SqnAct[Net#spl] == R[Net#a];
+  assert {:msg "  41.15: Action at 14.3 ('normal') for actor instance 'adj' might not preserve the channel invariant (#135)"} SqnAct[Net#pri] == R[Net#b];
+  assert {:msg "  42.15: Action at 14.3 ('normal') for actor instance 'adj' might not preserve the channel invariant (#136)"} SqnAct[Net#sec] == R[Net#c];
+  assert {:msg "  43.15: Action at 14.3 ('normal') for actor instance 'adj' might not preserve the channel invariant (#137)"} SqnAct[Net#adj] == R[Net#e];
+  assert {:msg "  45.16: Action at 14.3 ('normal') for actor instance 'adj' might not preserve the channel invariant (#138)"} (forall i: int :: 
     (0 <= i) && (i < (R[Net#a] + C[Net#a])) ==> (SqnCh[Net#a][i] == i)
   );
-  assert {:msg "  46.3: Action at 14.3 ('normal') for actor instance 'adj' might not preserve the channel invariant (#235)"} (forall i: int :: 
+  assert {:msg "  46.16: Action at 14.3 ('normal') for actor instance 'adj' might not preserve the channel invariant (#139)"} (forall i: int :: 
     (0 <= i) && (i < (R[Net#b] + C[Net#b])) ==> (SqnCh[Net#b][i] == i)
   );
-  assert {:msg "  47.3: Action at 14.3 ('normal') for actor instance 'adj' might not preserve the channel invariant (#236)"} (forall i: int :: 
+  assert {:msg "  47.16: Action at 14.3 ('normal') for actor instance 'adj' might not preserve the channel invariant (#140)"} (forall i: int :: 
     (0 <= i) && (i < (R[Net#c] + C[Net#c])) ==> (SqnCh[Net#c][i] == i)
   );
-  assert {:msg "  48.3: Action at 14.3 ('normal') for actor instance 'adj' might not preserve the channel invariant (#237)"} (forall i: int :: 
+  assert {:msg "  48.16: Action at 14.3 ('normal') for actor instance 'adj' might not preserve the channel invariant (#141)"} (forall i: int :: 
     (0 <= i) && (i < (R[Net#d] + C[Net#d])) ==> (SqnCh[Net#d][i] == i)
   );
-  assert {:msg "  49.3: Action at 14.3 ('normal') for actor instance 'adj' might not preserve the channel invariant (#238)"} (forall i: int :: 
+  assert {:msg "  49.16: Action at 14.3 ('normal') for actor instance 'adj' might not preserve the channel invariant (#142)"} (forall i: int :: 
     (0 <= i) && (i < (R[Net#e] + C[Net#e])) ==> (SqnCh[Net#e][i] == i)
   );
-  assert {:msg "  50.3: Action at 14.3 ('normal') for actor instance 'adj' might not preserve the channel invariant (#239)"} (forall i: int :: 
+  assert {:msg "  50.16: Action at 14.3 ('normal') for actor instance 'adj' might not preserve the channel invariant (#143)"} (forall i: int :: 
     (0 <= i) && (i < (R[Net#g] + C[Net#g])) ==> (SqnCh[Net#g][i] == i)
   );
-  assert {:msg "  52.3: Action at 14.3 ('normal') for actor instance 'adj' might not preserve the channel invariant (#240)"} C[Net#f] == 1;
-  assert {:msg "  53.3: Action at 14.3 ('normal') for actor instance 'adj' might not preserve the channel invariant (#241)"} C[Net#g] == R[Net#e];
-  assert {:msg "  54.3: Action at 14.3 ('normal') for actor instance 'adj' might not preserve the channel invariant (#242)"} R[Net#e] == M[Net#f][R[Net#f]];
-  assert {:msg "  55.3: Action at 14.3 ('normal') for actor instance 'adj' might not preserve the channel invariant (#243)"} (forall i: int :: 
+  assert {:msg "  52.15: Action at 14.3 ('normal') for actor instance 'adj' might not preserve the channel invariant (#144)"} C[Net#f] == 1;
+  assert {:msg "  53.15: Action at 14.3 ('normal') for actor instance 'adj' might not preserve the channel invariant (#145)"} (R[Net#g] + C[Net#g]) == R[Net#e];
+  assert {:msg "  54.15: Action at 14.3 ('normal') for actor instance 'adj' might not preserve the channel invariant (#146)"} R[Net#e] == M[Net#f][R[Net#f]];
+  assert {:msg "  55.16: Action at 14.3 ('normal') for actor instance 'adj' might not preserve the channel invariant (#147)"} (forall i: int :: 
     (0 <= i) && (i < (R[Net#g] + C[Net#g])) ==> (SqnCh[Net#g][i] == i)
   );
-  assert {:msg "  59.3: Action at 14.3 ('normal') for actor instance 'adj' might not preserve the channel invariant (#244)"} (0 < R[Net#d]) && (0 < R[Net#e]) ==> (M[Net#d][R[Net#d] - 1] <= M[Net#e][R[Net#e] - 1]);
-  assert {:msg "  60.3: Action at 14.3 ('normal') for actor instance 'adj' might not preserve the channel invariant (#245)"} (forall i: int :: 
+  if ((0 < R[Net#d]) && (0 < R[Net#e])) {
+    assert {:msg "  57.42: Action at 14.3 ('normal') for actor instance 'adj' might not preserve the channel invariant (#148)"} M[Net#d][R[Net#d] - 1] <= M[Net#e][R[Net#e] - 1];
+  }
+  assert {:msg "  58.16: Action at 14.3 ('normal') for actor instance 'adj' might not preserve the channel invariant (#149)"} (forall i: int :: 
     (0 <= i) && (i < R[Net#e]) ==> (M[Net#g][i] == M[Net#e][i])
   );
 }
@@ -1012,54 +1306,107 @@ procedure Net#anon$3#Adjudicator#timeout#13()
   assume 0 <= C[Net#g];
   assume R[Net#g] == 0;
   assume R[Net#a] == (R[Net#b] + C[Net#b]);
+  assert {:msg "  "} R[Net#a] == (R[Net#b] + C[Net#b]);
   assume R[Net#a] == (R[Net#c] + C[Net#c]);
+  assert {:msg "  "} R[Net#a] == (R[Net#c] + C[Net#c]);
   assume R[Net#b] == (R[Net#d] + C[Net#d]);
+  assert {:msg "  "} R[Net#b] == (R[Net#d] + C[Net#d]);
   assume R[Net#c] == (R[Net#e] + C[Net#e]);
+  assert {:msg "  "} R[Net#c] == (R[Net#e] + C[Net#e]);
   assume (forall idx$: int :: 
+    (0 <= idx$) && (idx$ < (R[Net#b] + C[Net#b])) ==> (M[Net#b][idx$] == M[Net#a][idx$])
+  );
+  assert {:msg "  "} (forall idx$: int :: 
     (0 <= idx$) && (idx$ < (R[Net#b] + C[Net#b])) ==> (M[Net#b][idx$] == M[Net#a][idx$])
   );
   assume (forall idx$: int :: 
     (0 <= idx$) && (idx$ < (R[Net#c] + C[Net#c])) ==> (M[Net#c][idx$] == M[Net#a][idx$])
   );
+  assert {:msg "  "} (forall idx$: int :: 
+    (0 <= idx$) && (idx$ < (R[Net#c] + C[Net#c])) ==> (M[Net#c][idx$] == M[Net#a][idx$])
+  );
   assume (forall idx$: int :: 
+    (0 <= idx$) && (idx$ < (R[Net#d] + C[Net#d])) ==> (M[Net#d][idx$] == M[Net#b][idx$])
+  );
+  assert {:msg "  "} (forall idx$: int :: 
     (0 <= idx$) && (idx$ < (R[Net#d] + C[Net#d])) ==> (M[Net#d][idx$] == M[Net#b][idx$])
   );
   assume (forall idx$: int :: 
     (0 <= idx$) && (idx$ < (R[Net#e] + C[Net#e])) ==> (M[Net#e][idx$] == M[Net#c][idx$])
   );
+  assert {:msg "  "} (forall idx$: int :: 
+    (0 <= idx$) && (idx$ < (R[Net#e] + C[Net#e])) ==> (M[Net#e][idx$] == M[Net#c][idx$])
+  );
   assume (forall idx$: int :: 
     (0 <= idx$) && (idx$ < (R[Net#a] + C[Net#a])) ==> (SqnCh[Net#a][idx$] == idx$)
   );
+  assert {:msg "  "} (forall idx$: int :: 
+    (0 <= idx$) && (idx$ < (R[Net#a] + C[Net#a])) ==> (SqnCh[Net#a][idx$] == idx$)
+  );
   assume SqnAct[Net#spl] == R[Net#a];
+  assert {:msg "  40.15: "} SqnAct[Net#spl] == R[Net#a];
   assume SqnAct[Net#pri] == R[Net#b];
+  assert {:msg "  41.15: "} SqnAct[Net#pri] == R[Net#b];
   assume SqnAct[Net#sec] == R[Net#c];
+  assert {:msg "  42.15: "} SqnAct[Net#sec] == R[Net#c];
   assume SqnAct[Net#adj] == R[Net#e];
+  assert {:msg "  43.15: "} SqnAct[Net#adj] == R[Net#e];
   assume (forall i: int :: 
+    (0 <= i) && (i < (R[Net#a] + C[Net#a])) ==> (SqnCh[Net#a][i] == i)
+  );
+  assert {:msg "  45.16: "} (forall i: int :: 
     (0 <= i) && (i < (R[Net#a] + C[Net#a])) ==> (SqnCh[Net#a][i] == i)
   );
   assume (forall i: int :: 
     (0 <= i) && (i < (R[Net#b] + C[Net#b])) ==> (SqnCh[Net#b][i] == i)
   );
+  assert {:msg "  46.16: "} (forall i: int :: 
+    (0 <= i) && (i < (R[Net#b] + C[Net#b])) ==> (SqnCh[Net#b][i] == i)
+  );
   assume (forall i: int :: 
+    (0 <= i) && (i < (R[Net#c] + C[Net#c])) ==> (SqnCh[Net#c][i] == i)
+  );
+  assert {:msg "  47.16: "} (forall i: int :: 
     (0 <= i) && (i < (R[Net#c] + C[Net#c])) ==> (SqnCh[Net#c][i] == i)
   );
   assume (forall i: int :: 
     (0 <= i) && (i < (R[Net#d] + C[Net#d])) ==> (SqnCh[Net#d][i] == i)
   );
+  assert {:msg "  48.16: "} (forall i: int :: 
+    (0 <= i) && (i < (R[Net#d] + C[Net#d])) ==> (SqnCh[Net#d][i] == i)
+  );
   assume (forall i: int :: 
+    (0 <= i) && (i < (R[Net#e] + C[Net#e])) ==> (SqnCh[Net#e][i] == i)
+  );
+  assert {:msg "  49.16: "} (forall i: int :: 
     (0 <= i) && (i < (R[Net#e] + C[Net#e])) ==> (SqnCh[Net#e][i] == i)
   );
   assume (forall i: int :: 
     (0 <= i) && (i < (R[Net#g] + C[Net#g])) ==> (SqnCh[Net#g][i] == i)
   );
+  assert {:msg "  50.16: "} (forall i: int :: 
+    (0 <= i) && (i < (R[Net#g] + C[Net#g])) ==> (SqnCh[Net#g][i] == i)
+  );
   assume C[Net#f] == 1;
-  assume C[Net#g] == R[Net#e];
+  assert {:msg "  52.15: "} C[Net#f] == 1;
+  assume (R[Net#g] + C[Net#g]) == R[Net#e];
+  assert {:msg "  53.15: "} (R[Net#g] + C[Net#g]) == R[Net#e];
   assume R[Net#e] == M[Net#f][R[Net#f]];
+  assert {:msg "  54.15: "} R[Net#e] == M[Net#f][R[Net#f]];
   assume (forall i: int :: 
     (0 <= i) && (i < (R[Net#g] + C[Net#g])) ==> (SqnCh[Net#g][i] == i)
   );
-  assume (0 < R[Net#d]) && (0 < R[Net#e]) ==> (M[Net#d][R[Net#d] - 1] <= M[Net#e][R[Net#e] - 1]);
+  assert {:msg "  55.16: "} (forall i: int :: 
+    (0 <= i) && (i < (R[Net#g] + C[Net#g])) ==> (SqnCh[Net#g][i] == i)
+  );
+  if ((0 < R[Net#d]) && (0 < R[Net#e])) {
+    assume M[Net#d][R[Net#d] - 1] <= M[Net#e][R[Net#e] - 1];
+    assert {:msg "  57.42: "} M[Net#d][R[Net#d] - 1] <= M[Net#e][R[Net#e] - 1];
+  }
   assume (forall i: int :: 
+    (0 <= i) && (i < R[Net#e]) ==> (M[Net#g][i] == M[Net#e][i])
+  );
+  assert {:msg "  58.16: "} (forall i: int :: 
     (0 <= i) && (i < R[Net#e]) ==> (M[Net#g][i] == M[Net#e][i])
   );
   assume true;
@@ -1077,71 +1424,57 @@ procedure Net#anon$3#Adjudicator#timeout#13()
   SqnCh[Net#f][R[Net#f] + C[Net#f]] := SqnAct[Net#adj];
   C[Net#f] := C[Net#f] + 1;
   SqnAct[Net#adj] := SqnAct[Net#adj] + 1;
-  assume 0 <= R[Net#a];
-  assume 0 <= C[Net#a];
-  assume (R[Net#a] + C[Net#a]) <= L[Net#a];
-  assume 0 <= R[Net#b];
-  assume 0 <= C[Net#b];
-  assume 0 <= R[Net#c];
-  assume 0 <= C[Net#c];
-  assume 0 <= R[Net#d];
-  assume 0 <= C[Net#d];
-  assume 0 <= R[Net#e];
-  assume 0 <= C[Net#e];
-  assume 0 <= R[Net#f];
-  assume 0 <= C[Net#f];
-  assume 0 <= R[Net#g];
-  assume 0 <= C[Net#g];
-  assume R[Net#g] == 0;
-  assert {:msg "  Action at 18.3 ('timeout') for actor instance 'adj' might not preserve the channel invariant (#262)"} R[Net#a] == (R[Net#b] + C[Net#b]);
-  assert {:msg "  Action at 18.3 ('timeout') for actor instance 'adj' might not preserve the channel invariant (#263)"} R[Net#a] == (R[Net#c] + C[Net#c]);
-  assert {:msg "  Action at 18.3 ('timeout') for actor instance 'adj' might not preserve the channel invariant (#264)"} R[Net#b] == (R[Net#d] + C[Net#d]);
-  assert {:msg "  Action at 18.3 ('timeout') for actor instance 'adj' might not preserve the channel invariant (#265)"} R[Net#c] == (R[Net#e] + C[Net#e]);
-  assert {:msg "  Action at 18.3 ('timeout') for actor instance 'adj' might not preserve the channel invariant (#266)"} (forall idx$: int :: 
+  assert {:msg "  Action at 18.3 ('timeout') for actor instance 'adj' might not preserve the channel invariant (#150)"} R[Net#a] == (R[Net#b] + C[Net#b]);
+  assert {:msg "  Action at 18.3 ('timeout') for actor instance 'adj' might not preserve the channel invariant (#151)"} R[Net#a] == (R[Net#c] + C[Net#c]);
+  assert {:msg "  Action at 18.3 ('timeout') for actor instance 'adj' might not preserve the channel invariant (#152)"} R[Net#b] == (R[Net#d] + C[Net#d]);
+  assert {:msg "  Action at 18.3 ('timeout') for actor instance 'adj' might not preserve the channel invariant (#153)"} R[Net#c] == (R[Net#e] + C[Net#e]);
+  assert {:msg "  Action at 18.3 ('timeout') for actor instance 'adj' might not preserve the channel invariant (#154)"} (forall idx$: int :: 
     (0 <= idx$) && (idx$ < (R[Net#b] + C[Net#b])) ==> (M[Net#b][idx$] == M[Net#a][idx$])
   );
-  assert {:msg "  Action at 18.3 ('timeout') for actor instance 'adj' might not preserve the channel invariant (#267)"} (forall idx$: int :: 
+  assert {:msg "  Action at 18.3 ('timeout') for actor instance 'adj' might not preserve the channel invariant (#155)"} (forall idx$: int :: 
     (0 <= idx$) && (idx$ < (R[Net#c] + C[Net#c])) ==> (M[Net#c][idx$] == M[Net#a][idx$])
   );
-  assert {:msg "  Action at 18.3 ('timeout') for actor instance 'adj' might not preserve the channel invariant (#268)"} (forall idx$: int :: 
+  assert {:msg "  Action at 18.3 ('timeout') for actor instance 'adj' might not preserve the channel invariant (#156)"} (forall idx$: int :: 
     (0 <= idx$) && (idx$ < (R[Net#d] + C[Net#d])) ==> (M[Net#d][idx$] == M[Net#b][idx$])
   );
-  assert {:msg "  Action at 18.3 ('timeout') for actor instance 'adj' might not preserve the channel invariant (#269)"} (forall idx$: int :: 
+  assert {:msg "  Action at 18.3 ('timeout') for actor instance 'adj' might not preserve the channel invariant (#157)"} (forall idx$: int :: 
     (0 <= idx$) && (idx$ < (R[Net#e] + C[Net#e])) ==> (M[Net#e][idx$] == M[Net#c][idx$])
   );
-  assert {:msg "  Action at 18.3 ('timeout') for actor instance 'adj' might not preserve the channel invariant (#270)"} (forall idx$: int :: 
+  assert {:msg "  Action at 18.3 ('timeout') for actor instance 'adj' might not preserve the channel invariant (#158)"} (forall idx$: int :: 
     (0 <= idx$) && (idx$ < (R[Net#a] + C[Net#a])) ==> (SqnCh[Net#a][idx$] == idx$)
   );
-  assert {:msg "  40.3: Action at 18.3 ('timeout') for actor instance 'adj' might not preserve the channel invariant (#271)"} SqnAct[Net#spl] == R[Net#a];
-  assert {:msg "  41.3: Action at 18.3 ('timeout') for actor instance 'adj' might not preserve the channel invariant (#272)"} SqnAct[Net#pri] == R[Net#b];
-  assert {:msg "  42.3: Action at 18.3 ('timeout') for actor instance 'adj' might not preserve the channel invariant (#273)"} SqnAct[Net#sec] == R[Net#c];
-  assert {:msg "  43.3: Action at 18.3 ('timeout') for actor instance 'adj' might not preserve the channel invariant (#274)"} SqnAct[Net#adj] == R[Net#e];
-  assert {:msg "  45.3: Action at 18.3 ('timeout') for actor instance 'adj' might not preserve the channel invariant (#275)"} (forall i: int :: 
+  assert {:msg "  40.15: Action at 18.3 ('timeout') for actor instance 'adj' might not preserve the channel invariant (#159)"} SqnAct[Net#spl] == R[Net#a];
+  assert {:msg "  41.15: Action at 18.3 ('timeout') for actor instance 'adj' might not preserve the channel invariant (#160)"} SqnAct[Net#pri] == R[Net#b];
+  assert {:msg "  42.15: Action at 18.3 ('timeout') for actor instance 'adj' might not preserve the channel invariant (#161)"} SqnAct[Net#sec] == R[Net#c];
+  assert {:msg "  43.15: Action at 18.3 ('timeout') for actor instance 'adj' might not preserve the channel invariant (#162)"} SqnAct[Net#adj] == R[Net#e];
+  assert {:msg "  45.16: Action at 18.3 ('timeout') for actor instance 'adj' might not preserve the channel invariant (#163)"} (forall i: int :: 
     (0 <= i) && (i < (R[Net#a] + C[Net#a])) ==> (SqnCh[Net#a][i] == i)
   );
-  assert {:msg "  46.3: Action at 18.3 ('timeout') for actor instance 'adj' might not preserve the channel invariant (#276)"} (forall i: int :: 
+  assert {:msg "  46.16: Action at 18.3 ('timeout') for actor instance 'adj' might not preserve the channel invariant (#164)"} (forall i: int :: 
     (0 <= i) && (i < (R[Net#b] + C[Net#b])) ==> (SqnCh[Net#b][i] == i)
   );
-  assert {:msg "  47.3: Action at 18.3 ('timeout') for actor instance 'adj' might not preserve the channel invariant (#277)"} (forall i: int :: 
+  assert {:msg "  47.16: Action at 18.3 ('timeout') for actor instance 'adj' might not preserve the channel invariant (#165)"} (forall i: int :: 
     (0 <= i) && (i < (R[Net#c] + C[Net#c])) ==> (SqnCh[Net#c][i] == i)
   );
-  assert {:msg "  48.3: Action at 18.3 ('timeout') for actor instance 'adj' might not preserve the channel invariant (#278)"} (forall i: int :: 
+  assert {:msg "  48.16: Action at 18.3 ('timeout') for actor instance 'adj' might not preserve the channel invariant (#166)"} (forall i: int :: 
     (0 <= i) && (i < (R[Net#d] + C[Net#d])) ==> (SqnCh[Net#d][i] == i)
   );
-  assert {:msg "  49.3: Action at 18.3 ('timeout') for actor instance 'adj' might not preserve the channel invariant (#279)"} (forall i: int :: 
+  assert {:msg "  49.16: Action at 18.3 ('timeout') for actor instance 'adj' might not preserve the channel invariant (#167)"} (forall i: int :: 
     (0 <= i) && (i < (R[Net#e] + C[Net#e])) ==> (SqnCh[Net#e][i] == i)
   );
-  assert {:msg "  50.3: Action at 18.3 ('timeout') for actor instance 'adj' might not preserve the channel invariant (#280)"} (forall i: int :: 
+  assert {:msg "  50.16: Action at 18.3 ('timeout') for actor instance 'adj' might not preserve the channel invariant (#168)"} (forall i: int :: 
     (0 <= i) && (i < (R[Net#g] + C[Net#g])) ==> (SqnCh[Net#g][i] == i)
   );
-  assert {:msg "  52.3: Action at 18.3 ('timeout') for actor instance 'adj' might not preserve the channel invariant (#281)"} C[Net#f] == 1;
-  assert {:msg "  53.3: Action at 18.3 ('timeout') for actor instance 'adj' might not preserve the channel invariant (#282)"} C[Net#g] == R[Net#e];
-  assert {:msg "  54.3: Action at 18.3 ('timeout') for actor instance 'adj' might not preserve the channel invariant (#283)"} R[Net#e] == M[Net#f][R[Net#f]];
-  assert {:msg "  55.3: Action at 18.3 ('timeout') for actor instance 'adj' might not preserve the channel invariant (#284)"} (forall i: int :: 
+  assert {:msg "  52.15: Action at 18.3 ('timeout') for actor instance 'adj' might not preserve the channel invariant (#169)"} C[Net#f] == 1;
+  assert {:msg "  53.15: Action at 18.3 ('timeout') for actor instance 'adj' might not preserve the channel invariant (#170)"} (R[Net#g] + C[Net#g]) == R[Net#e];
+  assert {:msg "  54.15: Action at 18.3 ('timeout') for actor instance 'adj' might not preserve the channel invariant (#171)"} R[Net#e] == M[Net#f][R[Net#f]];
+  assert {:msg "  55.16: Action at 18.3 ('timeout') for actor instance 'adj' might not preserve the channel invariant (#172)"} (forall i: int :: 
     (0 <= i) && (i < (R[Net#g] + C[Net#g])) ==> (SqnCh[Net#g][i] == i)
   );
-  assert {:msg "  59.3: Action at 18.3 ('timeout') for actor instance 'adj' might not preserve the channel invariant (#285)"} (0 < R[Net#d]) && (0 < R[Net#e]) ==> (M[Net#d][R[Net#d] - 1] <= M[Net#e][R[Net#e] - 1]);
-  assert {:msg "  60.3: Action at 18.3 ('timeout') for actor instance 'adj' might not preserve the channel invariant (#286)"} (forall i: int :: 
+  if ((0 < R[Net#d]) && (0 < R[Net#e])) {
+    assert {:msg "  57.42: Action at 18.3 ('timeout') for actor instance 'adj' might not preserve the channel invariant (#173)"} M[Net#d][R[Net#d] - 1] <= M[Net#e][R[Net#e] - 1];
+  }
+  assert {:msg "  58.16: Action at 18.3 ('timeout') for actor instance 'adj' might not preserve the channel invariant (#174)"} (forall i: int :: 
     (0 <= i) && (i < R[Net#e]) ==> (M[Net#g][i] == M[Net#e][i])
   );
 }
@@ -1166,54 +1499,107 @@ procedure Net#anon$3#exit#14()
   assume 0 <= C[Net#g];
   assume R[Net#g] == 0;
   assume R[Net#a] == (R[Net#b] + C[Net#b]);
+  assert {:msg "  "} R[Net#a] == (R[Net#b] + C[Net#b]);
   assume R[Net#a] == (R[Net#c] + C[Net#c]);
+  assert {:msg "  "} R[Net#a] == (R[Net#c] + C[Net#c]);
   assume R[Net#b] == (R[Net#d] + C[Net#d]);
+  assert {:msg "  "} R[Net#b] == (R[Net#d] + C[Net#d]);
   assume R[Net#c] == (R[Net#e] + C[Net#e]);
+  assert {:msg "  "} R[Net#c] == (R[Net#e] + C[Net#e]);
   assume (forall idx$: int :: 
+    (0 <= idx$) && (idx$ < (R[Net#b] + C[Net#b])) ==> (M[Net#b][idx$] == M[Net#a][idx$])
+  );
+  assert {:msg "  "} (forall idx$: int :: 
     (0 <= idx$) && (idx$ < (R[Net#b] + C[Net#b])) ==> (M[Net#b][idx$] == M[Net#a][idx$])
   );
   assume (forall idx$: int :: 
     (0 <= idx$) && (idx$ < (R[Net#c] + C[Net#c])) ==> (M[Net#c][idx$] == M[Net#a][idx$])
   );
+  assert {:msg "  "} (forall idx$: int :: 
+    (0 <= idx$) && (idx$ < (R[Net#c] + C[Net#c])) ==> (M[Net#c][idx$] == M[Net#a][idx$])
+  );
   assume (forall idx$: int :: 
+    (0 <= idx$) && (idx$ < (R[Net#d] + C[Net#d])) ==> (M[Net#d][idx$] == M[Net#b][idx$])
+  );
+  assert {:msg "  "} (forall idx$: int :: 
     (0 <= idx$) && (idx$ < (R[Net#d] + C[Net#d])) ==> (M[Net#d][idx$] == M[Net#b][idx$])
   );
   assume (forall idx$: int :: 
     (0 <= idx$) && (idx$ < (R[Net#e] + C[Net#e])) ==> (M[Net#e][idx$] == M[Net#c][idx$])
   );
+  assert {:msg "  "} (forall idx$: int :: 
+    (0 <= idx$) && (idx$ < (R[Net#e] + C[Net#e])) ==> (M[Net#e][idx$] == M[Net#c][idx$])
+  );
   assume (forall idx$: int :: 
     (0 <= idx$) && (idx$ < (R[Net#a] + C[Net#a])) ==> (SqnCh[Net#a][idx$] == idx$)
   );
+  assert {:msg "  "} (forall idx$: int :: 
+    (0 <= idx$) && (idx$ < (R[Net#a] + C[Net#a])) ==> (SqnCh[Net#a][idx$] == idx$)
+  );
   assume SqnAct[Net#spl] == R[Net#a];
+  assert {:msg "  40.15: "} SqnAct[Net#spl] == R[Net#a];
   assume SqnAct[Net#pri] == R[Net#b];
+  assert {:msg "  41.15: "} SqnAct[Net#pri] == R[Net#b];
   assume SqnAct[Net#sec] == R[Net#c];
+  assert {:msg "  42.15: "} SqnAct[Net#sec] == R[Net#c];
   assume SqnAct[Net#adj] == R[Net#e];
+  assert {:msg "  43.15: "} SqnAct[Net#adj] == R[Net#e];
   assume (forall i: int :: 
+    (0 <= i) && (i < (R[Net#a] + C[Net#a])) ==> (SqnCh[Net#a][i] == i)
+  );
+  assert {:msg "  45.16: "} (forall i: int :: 
     (0 <= i) && (i < (R[Net#a] + C[Net#a])) ==> (SqnCh[Net#a][i] == i)
   );
   assume (forall i: int :: 
     (0 <= i) && (i < (R[Net#b] + C[Net#b])) ==> (SqnCh[Net#b][i] == i)
   );
+  assert {:msg "  46.16: "} (forall i: int :: 
+    (0 <= i) && (i < (R[Net#b] + C[Net#b])) ==> (SqnCh[Net#b][i] == i)
+  );
   assume (forall i: int :: 
+    (0 <= i) && (i < (R[Net#c] + C[Net#c])) ==> (SqnCh[Net#c][i] == i)
+  );
+  assert {:msg "  47.16: "} (forall i: int :: 
     (0 <= i) && (i < (R[Net#c] + C[Net#c])) ==> (SqnCh[Net#c][i] == i)
   );
   assume (forall i: int :: 
     (0 <= i) && (i < (R[Net#d] + C[Net#d])) ==> (SqnCh[Net#d][i] == i)
   );
+  assert {:msg "  48.16: "} (forall i: int :: 
+    (0 <= i) && (i < (R[Net#d] + C[Net#d])) ==> (SqnCh[Net#d][i] == i)
+  );
   assume (forall i: int :: 
+    (0 <= i) && (i < (R[Net#e] + C[Net#e])) ==> (SqnCh[Net#e][i] == i)
+  );
+  assert {:msg "  49.16: "} (forall i: int :: 
     (0 <= i) && (i < (R[Net#e] + C[Net#e])) ==> (SqnCh[Net#e][i] == i)
   );
   assume (forall i: int :: 
     (0 <= i) && (i < (R[Net#g] + C[Net#g])) ==> (SqnCh[Net#g][i] == i)
   );
+  assert {:msg "  50.16: "} (forall i: int :: 
+    (0 <= i) && (i < (R[Net#g] + C[Net#g])) ==> (SqnCh[Net#g][i] == i)
+  );
   assume C[Net#f] == 1;
-  assume C[Net#g] == R[Net#e];
+  assert {:msg "  52.15: "} C[Net#f] == 1;
+  assume (R[Net#g] + C[Net#g]) == R[Net#e];
+  assert {:msg "  53.15: "} (R[Net#g] + C[Net#g]) == R[Net#e];
   assume R[Net#e] == M[Net#f][R[Net#f]];
+  assert {:msg "  54.15: "} R[Net#e] == M[Net#f][R[Net#f]];
   assume (forall i: int :: 
     (0 <= i) && (i < (R[Net#g] + C[Net#g])) ==> (SqnCh[Net#g][i] == i)
   );
-  assume (0 < R[Net#d]) && (0 < R[Net#e]) ==> (M[Net#d][R[Net#d] - 1] <= M[Net#e][R[Net#e] - 1]);
+  assert {:msg "  55.16: "} (forall i: int :: 
+    (0 <= i) && (i < (R[Net#g] + C[Net#g])) ==> (SqnCh[Net#g][i] == i)
+  );
+  if ((0 < R[Net#d]) && (0 < R[Net#e])) {
+    assume M[Net#d][R[Net#d] - 1] <= M[Net#e][R[Net#e] - 1];
+    assert {:msg "  57.42: "} M[Net#d][R[Net#d] - 1] <= M[Net#e][R[Net#e] - 1];
+  }
   assume (forall i: int :: 
+    (0 <= i) && (i < R[Net#e]) ==> (M[Net#g][i] == M[Net#e][i])
+  );
+  assert {:msg "  58.16: "} (forall i: int :: 
     (0 <= i) && (i < R[Net#e]) ==> (M[Net#g][i] == M[Net#e][i])
   );
   assume !((R[Net#a] + C[Net#a]) < L[Net#a]);
@@ -1231,6 +1617,59 @@ procedure Net#anon$3#exit#14()
   );
   R[Net#g] := R[Net#g] + C[Net#g];
   C[Net#g] := C[Net#g] - (1 * Base#L);
+  assert {:msg "  The network might not preserve the channel invariant"} R[Net#a] == (R[Net#b] + C[Net#b]);
+  assert {:msg "  The network might not preserve the channel invariant"} R[Net#a] == (R[Net#c] + C[Net#c]);
+  assert {:msg "  The network might not preserve the channel invariant"} R[Net#b] == (R[Net#d] + C[Net#d]);
+  assert {:msg "  The network might not preserve the channel invariant"} R[Net#c] == (R[Net#e] + C[Net#e]);
+  assert {:msg "  The network might not preserve the channel invariant"} (forall idx$: int :: 
+    (0 <= idx$) && (idx$ < (R[Net#b] + C[Net#b])) ==> (M[Net#b][idx$] == M[Net#a][idx$])
+  );
+  assert {:msg "  The network might not preserve the channel invariant"} (forall idx$: int :: 
+    (0 <= idx$) && (idx$ < (R[Net#c] + C[Net#c])) ==> (M[Net#c][idx$] == M[Net#a][idx$])
+  );
+  assert {:msg "  The network might not preserve the channel invariant"} (forall idx$: int :: 
+    (0 <= idx$) && (idx$ < (R[Net#d] + C[Net#d])) ==> (M[Net#d][idx$] == M[Net#b][idx$])
+  );
+  assert {:msg "  The network might not preserve the channel invariant"} (forall idx$: int :: 
+    (0 <= idx$) && (idx$ < (R[Net#e] + C[Net#e])) ==> (M[Net#e][idx$] == M[Net#c][idx$])
+  );
+  assert {:msg "  The network might not preserve the channel invariant"} (forall idx$: int :: 
+    (0 <= idx$) && (idx$ < (R[Net#a] + C[Net#a])) ==> (SqnCh[Net#a][idx$] == idx$)
+  );
+  assert {:msg "  40.15: The network might not preserve the channel invariant"} SqnAct[Net#spl] == R[Net#a];
+  assert {:msg "  41.15: The network might not preserve the channel invariant"} SqnAct[Net#pri] == R[Net#b];
+  assert {:msg "  42.15: The network might not preserve the channel invariant"} SqnAct[Net#sec] == R[Net#c];
+  assert {:msg "  43.15: The network might not preserve the channel invariant"} SqnAct[Net#adj] == R[Net#e];
+  assert {:msg "  45.16: The network might not preserve the channel invariant"} (forall i: int :: 
+    (0 <= i) && (i < (R[Net#a] + C[Net#a])) ==> (SqnCh[Net#a][i] == i)
+  );
+  assert {:msg "  46.16: The network might not preserve the channel invariant"} (forall i: int :: 
+    (0 <= i) && (i < (R[Net#b] + C[Net#b])) ==> (SqnCh[Net#b][i] == i)
+  );
+  assert {:msg "  47.16: The network might not preserve the channel invariant"} (forall i: int :: 
+    (0 <= i) && (i < (R[Net#c] + C[Net#c])) ==> (SqnCh[Net#c][i] == i)
+  );
+  assert {:msg "  48.16: The network might not preserve the channel invariant"} (forall i: int :: 
+    (0 <= i) && (i < (R[Net#d] + C[Net#d])) ==> (SqnCh[Net#d][i] == i)
+  );
+  assert {:msg "  49.16: The network might not preserve the channel invariant"} (forall i: int :: 
+    (0 <= i) && (i < (R[Net#e] + C[Net#e])) ==> (SqnCh[Net#e][i] == i)
+  );
+  assert {:msg "  50.16: The network might not preserve the channel invariant"} (forall i: int :: 
+    (0 <= i) && (i < (R[Net#g] + C[Net#g])) ==> (SqnCh[Net#g][i] == i)
+  );
+  assert {:msg "  52.15: The network might not preserve the channel invariant"} C[Net#f] == 1;
+  assert {:msg "  53.15: The network might not preserve the channel invariant"} (R[Net#g] + C[Net#g]) == R[Net#e];
+  assert {:msg "  54.15: The network might not preserve the channel invariant"} R[Net#e] == M[Net#f][R[Net#f]];
+  assert {:msg "  55.16: The network might not preserve the channel invariant"} (forall i: int :: 
+    (0 <= i) && (i < (R[Net#g] + C[Net#g])) ==> (SqnCh[Net#g][i] == i)
+  );
+  if ((0 < R[Net#d]) && (0 < R[Net#e])) {
+    assert {:msg "  57.42: The network might not preserve the channel invariant"} M[Net#d][R[Net#d] - 1] <= M[Net#e][R[Net#e] - 1];
+  }
+  assert {:msg "  58.16: The network might not preserve the channel invariant"} (forall i: int :: 
+    (0 <= i) && (i < R[Net#e]) ==> (M[Net#g][i] == M[Net#e][i])
+  );
   C[Net#f] := C[Net#f] - 1;
   assert {:msg "  38.13: The network might not preserve the network invariant"} R[Net#e] == M[Net#f][R[Net#f]];
   assert {:msg "  32.3: The network might leave unread tokens on channel a"} C[Net#a] == 0;
