tests/AddDelay.bpl
@@ -21,7 +21,6 @@ var AT#intlst: List int;
 
 function AT#Min(x:int, y: int): int { if x <= y then x else y }
 
-
 // ---------------------------------------------------------------
 // -- End of prelude ---------------------------------------------
 // ---------------------------------------------------------------
@@ -29,21 +28,25 @@ function AT#Min(x:int, y: int): int { if x <= y then x else y }
 procedure Add#anon$0#0()
   modifies C, R, M, St;
 {
-  var IV#in1#0: int;
-  var IV#in2#0: int;
+  var in1: Chan (int);
+  var in2: Chan (int);
+  var out: Chan (int);
   assume true;
   assume true;
 }
 procedure Delay#anon$1#1()
   modifies C, R, M, St;
 {
+  var in: Chan (int);
+  var out: Chan (int);
   assume true;
   assume true;
 }
 procedure Delay#anon$2#2()
   modifies C, R, M, St;
 {
-  var IV#in#0: int;
+  var in: Chan (int);
+  var out: Chan (int);
   assume true;
   assume true;
 }
@@ -74,19 +77,14 @@ const unique Net#d: Chan (int);
 procedure Net#anon$3#entry#4()
   modifies C, R, M, St;
 {
-  var ActionPH#y: int;
   assume L[Net#a] == (1 * Base#L);
-  assume R[Net#a] == 0;
   assume C[Net#a] == 0;
-  assume R[Net#b] == 0;
   assume C[Net#b] == 0;
-  assume R[Net#c] == 0;
   assume C[Net#c] == 0;
-  assume R[Net#d] == 0;
   assume C[Net#d] == 0;
   C[Net#b] := C[Net#b] + 1;
   assume (M[Net#b][R[Net#b]] == M[Net#c][R[Net#c] - 1]) || (M[Net#b][R[Net#b]] == 0);
-  assume 0 < M[Net#a][0];
+  assert {:msg "  25.13: Invariant might not hold"} (M[Net#b][R[Net#b]] == M[Net#c][R[Net#c] - 1]) || (M[Net#b][R[Net#b]] == 0);
   assume 0 <= R[Net#a];
   assume 0 <= C[Net#a];
   assume (R[Net#a] + C[Net#a]) <= L[Net#a];
@@ -97,27 +95,56 @@ procedure Net#anon$3#entry#4()
   assume R[Net#c] == 0;
   assume 0 <= R[Net#d];
   assume 0 <= C[Net#d];
-  assert {:msg "  Channel invariant might not hold on action entry (#10)"} 0 < M[Net#a][0];
-  assert {:msg "  Channel invariant might not hold on action entry (#11)"} R[Net#a] == (R[Net#c] + C[Net#c]);
-  assert {:msg "  Channel invariant might not hold on action entry (#12)"} R[Net#b] == (R[Net#c] + C[Net#c]);
-  assert {:msg "  Channel invariant might not hold on action entry (#13)"} R[Net#a] == (R[Net#d] + C[Net#d]);
-  assert {:msg "  Channel invariant might not hold on action entry (#14)"} R[Net#b] == (R[Net#d] + C[Net#d]);
-  assert {:msg "  Channel invariant might not hold on action entry (#15)"} R[Net#d] == ((R[Net#b] + C[Net#b]) - 1);
-  assert {:msg "  Channel invariant might not hold on action entry (#16)"} (forall idx$: int :: 
+  assume R[Net#a] == (R[Net#c] + C[Net#c]);
+  assert {:msg "  Invariant might not hold"} R[Net#a] == (R[Net#c] + C[Net#c]);
+  assume R[Net#b] == (R[Net#c] + C[Net#c]);
+  assert {:msg "  Invariant might not hold"} R[Net#b] == (R[Net#c] + C[Net#c]);
+  assume R[Net#a] == (R[Net#d] + C[Net#d]);
+  assert {:msg "  Invariant might not hold"} R[Net#a] == (R[Net#d] + C[Net#d]);
+  assume R[Net#b] == (R[Net#d] + C[Net#d]);
+  assert {:msg "  Invariant might not hold"} R[Net#b] == (R[Net#d] + C[Net#d]);
+  assume R[Net#d] == ((R[Net#b] + C[Net#b]) - 1);
+  assert {:msg "  Invariant might not hold"} R[Net#d] == ((R[Net#b] + C[Net#b]) - 1);
+  assume (forall idx$: int :: 
     (0 <= idx$) && (idx$ < (R[Net#c] + C[Net#c])) ==> (M[Net#c][idx$] == (M[Net#a][idx$] + M[Net#b][idx$]))
   );
-  assert {:msg "  Channel invariant might not hold on action entry (#17)"} (forall idx$: int :: 
+  assert {:msg "  Invariant might not hold"} (forall idx$: int :: 
+    (0 <= idx$) && (idx$ < (R[Net#c] + C[Net#c])) ==> (M[Net#c][idx$] == (M[Net#a][idx$] + M[Net#b][idx$]))
+  );
+  assume (forall idx$: int :: 
     (0 <= idx$) && (idx$ < (R[Net#d] + C[Net#d])) ==> (M[Net#d][idx$] == (M[Net#a][idx$] + M[Net#b][idx$]))
   );
-  assert {:msg "  Channel invariant might not hold on action entry (#18)"} (forall idx$: int :: 
+  assert {:msg "  Invariant might not hold"} (forall idx$: int :: 
+    (0 <= idx$) && (idx$ < (R[Net#d] + C[Net#d])) ==> (M[Net#d][idx$] == (M[Net#a][idx$] + M[Net#b][idx$]))
+  );
+  assume (forall idx$: int :: 
     (1 <= idx$) && (idx$ < (R[Net#b] + C[Net#b])) ==> (M[Net#b][idx$] == M[Net#d][idx$ - 1])
   );
-  assert {:msg "  27.3: Channel invariant might not hold on action entry (#19)"} (M[Net#b][0] == M[Net#c][-1]) || (M[Net#b][0] == 0);
+  assert {:msg "  Invariant might not hold"} (forall idx$: int :: 
+    (1 <= idx$) && (idx$ < (R[Net#b] + C[Net#b])) ==> (M[Net#b][idx$] == M[Net#d][idx$ - 1])
+  );
+  assume (M[Net#b][0] == M[Net#c][-1]) || (M[Net#b][0] == 0);
+  assert {:msg "  27.15: Invariant might not hold"} (M[Net#b][0] == M[Net#c][-1]) || (M[Net#b][0] == 0);
+  assume 0 < M[Net#a][0];
+  assert {:msg "  Channel invariant might not hold on action entry (#0)"} R[Net#a] == (R[Net#c] + C[Net#c]);
+  assert {:msg "  Channel invariant might not hold on action entry (#1)"} R[Net#b] == (R[Net#c] + C[Net#c]);
+  assert {:msg "  Channel invariant might not hold on action entry (#2)"} R[Net#a] == (R[Net#d] + C[Net#d]);
+  assert {:msg "  Channel invariant might not hold on action entry (#3)"} R[Net#b] == (R[Net#d] + C[Net#d]);
+  assert {:msg "  Channel invariant might not hold on action entry (#4)"} R[Net#d] == ((R[Net#b] + C[Net#b]) - 1);
+  assert {:msg "  Channel invariant might not hold on action entry (#5)"} (forall idx$: int :: 
+    (0 <= idx$) && (idx$ < (R[Net#c] + C[Net#c])) ==> (M[Net#c][idx$] == (M[Net#a][idx$] + M[Net#b][idx$]))
+  );
+  assert {:msg "  Channel invariant might not hold on action entry (#6)"} (forall idx$: int :: 
+    (0 <= idx$) && (idx$ < (R[Net#d] + C[Net#d])) ==> (M[Net#d][idx$] == (M[Net#a][idx$] + M[Net#b][idx$]))
+  );
+  assert {:msg "  Channel invariant might not hold on action entry (#7)"} (forall idx$: int :: 
+    (1 <= idx$) && (idx$ < (R[Net#b] + C[Net#b])) ==> (M[Net#b][idx$] == M[Net#d][idx$ - 1])
+  );
+  assert {:msg "  27.15: Channel invariant might not hold on action entry (#8)"} (M[Net#b][0] == M[Net#c][-1]) || (M[Net#b][0] == 0);
 }
 procedure Net#anon$3#Add#anon$0#5()
   modifies C, R, M, St;
 {
-  var ActionPH#y: int;
   var St#next: State;
   var in1#i: int;
   var in2#j: int;
@@ -132,22 +159,36 @@ procedure Net#anon$3#Add#anon$0#5()
   assume R[Net#c] == 0;
   assume 0 <= R[Net#d];
   assume 0 <= C[Net#d];
-  assume 0 < M[Net#a][0];
   assume R[Net#a] == (R[Net#c] + C[Net#c]);
+  assert {:msg "  "} R[Net#a] == (R[Net#c] + C[Net#c]);
   assume R[Net#b] == (R[Net#c] + C[Net#c]);
+  assert {:msg "  "} R[Net#b] == (R[Net#c] + C[Net#c]);
   assume R[Net#a] == (R[Net#d] + C[Net#d]);
+  assert {:msg "  "} R[Net#a] == (R[Net#d] + C[Net#d]);
   assume R[Net#b] == (R[Net#d] + C[Net#d]);
+  assert {:msg "  "} R[Net#b] == (R[Net#d] + C[Net#d]);
   assume R[Net#d] == ((R[Net#b] + C[Net#b]) - 1);
+  assert {:msg "  "} R[Net#d] == ((R[Net#b] + C[Net#b]) - 1);
   assume (forall idx$: int :: 
+    (0 <= idx$) && (idx$ < (R[Net#c] + C[Net#c])) ==> (M[Net#c][idx$] == (M[Net#a][idx$] + M[Net#b][idx$]))
+  );
+  assert {:msg "  "} (forall idx$: int :: 
     (0 <= idx$) && (idx$ < (R[Net#c] + C[Net#c])) ==> (M[Net#c][idx$] == (M[Net#a][idx$] + M[Net#b][idx$]))
   );
   assume (forall idx$: int :: 
     (0 <= idx$) && (idx$ < (R[Net#d] + C[Net#d])) ==> (M[Net#d][idx$] == (M[Net#a][idx$] + M[Net#b][idx$]))
   );
+  assert {:msg "  "} (forall idx$: int :: 
+    (0 <= idx$) && (idx$ < (R[Net#d] + C[Net#d])) ==> (M[Net#d][idx$] == (M[Net#a][idx$] + M[Net#b][idx$]))
+  );
   assume (forall idx$: int :: 
     (1 <= idx$) && (idx$ < (R[Net#b] + C[Net#b])) ==> (M[Net#b][idx$] == M[Net#d][idx$ - 1])
   );
+  assert {:msg "  "} (forall idx$: int :: 
+    (1 <= idx$) && (idx$ < (R[Net#b] + C[Net#b])) ==> (M[Net#b][idx$] == M[Net#d][idx$ - 1])
+  );
   assume (M[Net#b][0] == M[Net#c][-1]) || (M[Net#b][0] == 0);
+  assert {:msg "  27.15: "} (M[Net#b][0] == M[Net#c][-1]) || (M[Net#b][0] == 0);
   assume true;
   assume (1 <= C[Net#a]) && (1 <= C[Net#b]);
   in1#i := M[Net#a][R[Net#a]];
@@ -160,37 +201,25 @@ procedure Net#anon$3#Add#anon$0#5()
   C[Net#c] := C[Net#c] + 1;
   M[Net#d][R[Net#d] + C[Net#d]] := in1#i + in2#j;
   C[Net#d] := C[Net#d] + 1;
-  assume 0 <= R[Net#a];
-  assume 0 <= C[Net#a];
-  assume (R[Net#a] + C[Net#a]) <= L[Net#a];
-  assume 0 <= R[Net#b];
-  assume 0 <= C[Net#b];
-  assume 0 <= R[Net#c];
-  assume 0 <= C[Net#c];
-  assume R[Net#c] == 0;
-  assume 0 <= R[Net#d];
-  assume 0 <= C[Net#d];
-  assert {:msg "  Action at 3.3 ('anon$0') for actor instance 'add' might not preserve the channel invariant (#30)"} 0 < M[Net#a][0];
-  assert {:msg "  Action at 3.3 ('anon$0') for actor instance 'add' might not preserve the channel invariant (#31)"} R[Net#a] == (R[Net#c] + C[Net#c]);
-  assert {:msg "  Action at 3.3 ('anon$0') for actor instance 'add' might not preserve the channel invariant (#32)"} R[Net#b] == (R[Net#c] + C[Net#c]);
-  assert {:msg "  Action at 3.3 ('anon$0') for actor instance 'add' might not preserve the channel invariant (#33)"} R[Net#a] == (R[Net#d] + C[Net#d]);
-  assert {:msg "  Action at 3.3 ('anon$0') for actor instance 'add' might not preserve the channel invariant (#34)"} R[Net#b] == (R[Net#d] + C[Net#d]);
-  assert {:msg "  Action at 3.3 ('anon$0') for actor instance 'add' might not preserve the channel invariant (#35)"} R[Net#d] == ((R[Net#b] + C[Net#b]) - 1);
-  assert {:msg "  Action at 3.3 ('anon$0') for actor instance 'add' might not preserve the channel invariant (#36)"} (forall idx$: int :: 
+  assert {:msg "  Action at 3.3 ('anon$0') for actor instance 'add' might not preserve the channel invariant (#9)"} R[Net#a] == (R[Net#c] + C[Net#c]);
+  assert {:msg "  Action at 3.3 ('anon$0') for actor instance 'add' might not preserve the channel invariant (#10)"} R[Net#b] == (R[Net#c] + C[Net#c]);
+  assert {:msg "  Action at 3.3 ('anon$0') for actor instance 'add' might not preserve the channel invariant (#11)"} R[Net#a] == (R[Net#d] + C[Net#d]);
+  assert {:msg "  Action at 3.3 ('anon$0') for actor instance 'add' might not preserve the channel invariant (#12)"} R[Net#b] == (R[Net#d] + C[Net#d]);
+  assert {:msg "  Action at 3.3 ('anon$0') for actor instance 'add' might not preserve the channel invariant (#13)"} R[Net#d] == ((R[Net#b] + C[Net#b]) - 1);
+  assert {:msg "  Action at 3.3 ('anon$0') for actor instance 'add' might not preserve the channel invariant (#14)"} (forall idx$: int :: 
     (0 <= idx$) && (idx$ < (R[Net#c] + C[Net#c])) ==> (M[Net#c][idx$] == (M[Net#a][idx$] + M[Net#b][idx$]))
   );
-  assert {:msg "  Action at 3.3 ('anon$0') for actor instance 'add' might not preserve the channel invariant (#37)"} (forall idx$: int :: 
+  assert {:msg "  Action at 3.3 ('anon$0') for actor instance 'add' might not preserve the channel invariant (#15)"} (forall idx$: int :: 
     (0 <= idx$) && (idx$ < (R[Net#d] + C[Net#d])) ==> (M[Net#d][idx$] == (M[Net#a][idx$] + M[Net#b][idx$]))
   );
-  assert {:msg "  Action at 3.3 ('anon$0') for actor instance 'add' might not preserve the channel invariant (#38)"} (forall idx$: int :: 
+  assert {:msg "  Action at 3.3 ('anon$0') for actor instance 'add' might not preserve the channel invariant (#16)"} (forall idx$: int :: 
     (1 <= idx$) && (idx$ < (R[Net#b] + C[Net#b])) ==> (M[Net#b][idx$] == M[Net#d][idx$ - 1])
   );
-  assert {:msg "  27.3: Action at 3.3 ('anon$0') for actor instance 'add' might not preserve the channel invariant (#39)"} (M[Net#b][0] == M[Net#c][-1]) || (M[Net#b][0] == 0);
+  assert {:msg "  27.15: Action at 3.3 ('anon$0') for actor instance 'add' might not preserve the channel invariant (#17)"} (M[Net#b][0] == M[Net#c][-1]) || (M[Net#b][0] == 0);
 }
 procedure Net#anon$3#Delay#anon$2#6()
   modifies C, R, M, St;
 {
-  var ActionPH#y: int;
   var ActorParam#k: int;
   var St#next: State;
   var in#i: int;
@@ -206,22 +235,36 @@ procedure Net#anon$3#Delay#anon$2#6()
   assume R[Net#c] == 0;
   assume 0 <= R[Net#d];
   assume 0 <= C[Net#d];
-  assume 0 < M[Net#a][0];
   assume R[Net#a] == (R[Net#c] + C[Net#c]);
+  assert {:msg "  "} R[Net#a] == (R[Net#c] + C[Net#c]);
   assume R[Net#b] == (R[Net#c] + C[Net#c]);
+  assert {:msg "  "} R[Net#b] == (R[Net#c] + C[Net#c]);
   assume R[Net#a] == (R[Net#d] + C[Net#d]);
+  assert {:msg "  "} R[Net#a] == (R[Net#d] + C[Net#d]);
   assume R[Net#b] == (R[Net#d] + C[Net#d]);
+  assert {:msg "  "} R[Net#b] == (R[Net#d] + C[Net#d]);
   assume R[Net#d] == ((R[Net#b] + C[Net#b]) - 1);
+  assert {:msg "  "} R[Net#d] == ((R[Net#b] + C[Net#b]) - 1);
   assume (forall idx$: int :: 
+    (0 <= idx$) && (idx$ < (R[Net#c] + C[Net#c])) ==> (M[Net#c][idx$] == (M[Net#a][idx$] + M[Net#b][idx$]))
+  );
+  assert {:msg "  "} (forall idx$: int :: 
     (0 <= idx$) && (idx$ < (R[Net#c] + C[Net#c])) ==> (M[Net#c][idx$] == (M[Net#a][idx$] + M[Net#b][idx$]))
   );
   assume (forall idx$: int :: 
     (0 <= idx$) && (idx$ < (R[Net#d] + C[Net#d])) ==> (M[Net#d][idx$] == (M[Net#a][idx$] + M[Net#b][idx$]))
   );
+  assert {:msg "  "} (forall idx$: int :: 
+    (0 <= idx$) && (idx$ < (R[Net#d] + C[Net#d])) ==> (M[Net#d][idx$] == (M[Net#a][idx$] + M[Net#b][idx$]))
+  );
   assume (forall idx$: int :: 
     (1 <= idx$) && (idx$ < (R[Net#b] + C[Net#b])) ==> (M[Net#b][idx$] == M[Net#d][idx$ - 1])
   );
+  assert {:msg "  "} (forall idx$: int :: 
+    (1 <= idx$) && (idx$ < (R[Net#b] + C[Net#b])) ==> (M[Net#b][idx$] == M[Net#d][idx$ - 1])
+  );
   assume (M[Net#b][0] == M[Net#c][-1]) || (M[Net#b][0] == 0);
+  assert {:msg "  27.15: "} (M[Net#b][0] == M[Net#c][-1]) || (M[Net#b][0] == 0);
   assume true;
   assume 1 <= C[Net#d];
   in#i := M[Net#d][R[Net#d]];
@@ -229,37 +272,25 @@ procedure Net#anon$3#Delay#anon$2#6()
   C[Net#d] := C[Net#d] - 1;
   M[Net#b][R[Net#b] + C[Net#b]] := in#i;
   C[Net#b] := C[Net#b] + 1;
-  assume 0 <= R[Net#a];
-  assume 0 <= C[Net#a];
-  assume (R[Net#a] + C[Net#a]) <= L[Net#a];
-  assume 0 <= R[Net#b];
-  assume 0 <= C[Net#b];
-  assume 0 <= R[Net#c];
-  assume 0 <= C[Net#c];
-  assume R[Net#c] == 0;
-  assume 0 <= R[Net#d];
-  assume 0 <= C[Net#d];
-  assert {:msg "  Action at 9.3 ('anon$2') for actor instance 'del' might not preserve the channel invariant (#50)"} 0 < M[Net#a][0];
-  assert {:msg "  Action at 9.3 ('anon$2') for actor instance 'del' might not preserve the channel invariant (#51)"} R[Net#a] == (R[Net#c] + C[Net#c]);
-  assert {:msg "  Action at 9.3 ('anon$2') for actor instance 'del' might not preserve the channel invariant (#52)"} R[Net#b] == (R[Net#c] + C[Net#c]);
-  assert {:msg "  Action at 9.3 ('anon$2') for actor instance 'del' might not preserve the channel invariant (#53)"} R[Net#a] == (R[Net#d] + C[Net#d]);
-  assert {:msg "  Action at 9.3 ('anon$2') for actor instance 'del' might not preserve the channel invariant (#54)"} R[Net#b] == (R[Net#d] + C[Net#d]);
-  assert {:msg "  Action at 9.3 ('anon$2') for actor instance 'del' might not preserve the channel invariant (#55)"} R[Net#d] == ((R[Net#b] + C[Net#b]) - 1);
-  assert {:msg "  Action at 9.3 ('anon$2') for actor instance 'del' might not preserve the channel invariant (#56)"} (forall idx$: int :: 
+  assert {:msg "  Action at 9.3 ('anon$2') for actor instance 'del' might not preserve the channel invariant (#18)"} R[Net#a] == (R[Net#c] + C[Net#c]);
+  assert {:msg "  Action at 9.3 ('anon$2') for actor instance 'del' might not preserve the channel invariant (#19)"} R[Net#b] == (R[Net#c] + C[Net#c]);
+  assert {:msg "  Action at 9.3 ('anon$2') for actor instance 'del' might not preserve the channel invariant (#20)"} R[Net#a] == (R[Net#d] + C[Net#d]);
+  assert {:msg "  Action at 9.3 ('anon$2') for actor instance 'del' might not preserve the channel invariant (#21)"} R[Net#b] == (R[Net#d] + C[Net#d]);
+  assert {:msg "  Action at 9.3 ('anon$2') for actor instance 'del' might not preserve the channel invariant (#22)"} R[Net#d] == ((R[Net#b] + C[Net#b]) - 1);
+  assert {:msg "  Action at 9.3 ('anon$2') for actor instance 'del' might not preserve the channel invariant (#23)"} (forall idx$: int :: 
     (0 <= idx$) && (idx$ < (R[Net#c] + C[Net#c])) ==> (M[Net#c][idx$] == (M[Net#a][idx$] + M[Net#b][idx$]))
   );
-  assert {:msg "  Action at 9.3 ('anon$2') for actor instance 'del' might not preserve the channel invariant (#57)"} (forall idx$: int :: 
+  assert {:msg "  Action at 9.3 ('anon$2') for actor instance 'del' might not preserve the channel invariant (#24)"} (forall idx$: int :: 
     (0 <= idx$) && (idx$ < (R[Net#d] + C[Net#d])) ==> (M[Net#d][idx$] == (M[Net#a][idx$] + M[Net#b][idx$]))
   );
-  assert {:msg "  Action at 9.3 ('anon$2') for actor instance 'del' might not preserve the channel invariant (#58)"} (forall idx$: int :: 
+  assert {:msg "  Action at 9.3 ('anon$2') for actor instance 'del' might not preserve the channel invariant (#25)"} (forall idx$: int :: 
     (1 <= idx$) && (idx$ < (R[Net#b] + C[Net#b])) ==> (M[Net#b][idx$] == M[Net#d][idx$ - 1])
   );
-  assert {:msg "  27.3: Action at 9.3 ('anon$2') for actor instance 'del' might not preserve the channel invariant (#59)"} (M[Net#b][0] == M[Net#c][-1]) || (M[Net#b][0] == 0);
+  assert {:msg "  27.15: Action at 9.3 ('anon$2') for actor instance 'del' might not preserve the channel invariant (#26)"} (M[Net#b][0] == M[Net#c][-1]) || (M[Net#b][0] == 0);
 }
 procedure Net#anon$3#exit#7()
   modifies C, R, M, St;
 {
-  var ActionPH#y: int;
   assume L[Net#a] == (1 * Base#L);
   assume 0 <= R[Net#a];
   assume 0 <= C[Net#a];
@@ -271,29 +302,57 @@ procedure Net#anon$3#exit#7()
   assume R[Net#c] == 0;
   assume 0 <= R[Net#d];
   assume 0 <= C[Net#d];
-  assume 0 < M[Net#a][0];
   assume R[Net#a] == (R[Net#c] + C[Net#c]);
+  assert {:msg "  "} R[Net#a] == (R[Net#c] + C[Net#c]);
   assume R[Net#b] == (R[Net#c] + C[Net#c]);
+  assert {:msg "  "} R[Net#b] == (R[Net#c] + C[Net#c]);
   assume R[Net#a] == (R[Net#d] + C[Net#d]);
+  assert {:msg "  "} R[Net#a] == (R[Net#d] + C[Net#d]);
   assume R[Net#b] == (R[Net#d] + C[Net#d]);
+  assert {:msg "  "} R[Net#b] == (R[Net#d] + C[Net#d]);
   assume R[Net#d] == ((R[Net#b] + C[Net#b]) - 1);
+  assert {:msg "  "} R[Net#d] == ((R[Net#b] + C[Net#b]) - 1);
   assume (forall idx$: int :: 
+    (0 <= idx$) && (idx$ < (R[Net#c] + C[Net#c])) ==> (M[Net#c][idx$] == (M[Net#a][idx$] + M[Net#b][idx$]))
+  );
+  assert {:msg "  "} (forall idx$: int :: 
     (0 <= idx$) && (idx$ < (R[Net#c] + C[Net#c])) ==> (M[Net#c][idx$] == (M[Net#a][idx$] + M[Net#b][idx$]))
   );
   assume (forall idx$: int :: 
     (0 <= idx$) && (idx$ < (R[Net#d] + C[Net#d])) ==> (M[Net#d][idx$] == (M[Net#a][idx$] + M[Net#b][idx$]))
   );
+  assert {:msg "  "} (forall idx$: int :: 
+    (0 <= idx$) && (idx$ < (R[Net#d] + C[Net#d])) ==> (M[Net#d][idx$] == (M[Net#a][idx$] + M[Net#b][idx$]))
+  );
   assume (forall idx$: int :: 
     (1 <= idx$) && (idx$ < (R[Net#b] + C[Net#b])) ==> (M[Net#b][idx$] == M[Net#d][idx$ - 1])
   );
+  assert {:msg "  "} (forall idx$: int :: 
+    (1 <= idx$) && (idx$ < (R[Net#b] + C[Net#b])) ==> (M[Net#b][idx$] == M[Net#d][idx$ - 1])
+  );
   assume (M[Net#b][0] == M[Net#c][-1]) || (M[Net#b][0] == 0);
+  assert {:msg "  27.15: "} (M[Net#b][0] == M[Net#c][-1]) || (M[Net#b][0] == 0);
   assume !((R[Net#a] + C[Net#a]) < L[Net#a]);
   assume !((1 <= C[Net#a]) && (1 <= C[Net#b]));
   assume !(1 <= C[Net#d]);
-  ActionPH#y := M[Net#c][0];
-  assert {:msg "  21.13: Network action postcondition might not hold"} (ActionPH#y == (M[Net#c][R[Net#c] - 1] + M[Net#a][0])) || (ActionPH#y == M[Net#a][0]);
+  assert {:msg "  21.13: Network action postcondition might not hold"} (M[Net#c][0] == (M[Net#c][R[Net#c] - 1] + M[Net#a][0])) || (M[Net#c][0] == M[Net#a][0]);
   R[Net#c] := R[Net#c] + C[Net#c];
   C[Net#c] := C[Net#c] - (1 * Base#L);
+  assert {:msg "  The network might not preserve the channel invariant"} R[Net#a] == (R[Net#c] + C[Net#c]);
+  assert {:msg "  The network might not preserve the channel invariant"} R[Net#b] == (R[Net#c] + C[Net#c]);
+  assert {:msg "  The network might not preserve the channel invariant"} R[Net#a] == (R[Net#d] + C[Net#d]);
+  assert {:msg "  The network might not preserve the channel invariant"} R[Net#b] == (R[Net#d] + C[Net#d]);
+  assert {:msg "  The network might not preserve the channel invariant"} R[Net#d] == ((R[Net#b] + C[Net#b]) - 1);
+  assert {:msg "  The network might not preserve the channel invariant"} (forall idx$: int :: 
+    (0 <= idx$) && (idx$ < (R[Net#c] + C[Net#c])) ==> (M[Net#c][idx$] == (M[Net#a][idx$] + M[Net#b][idx$]))
+  );
+  assert {:msg "  The network might not preserve the channel invariant"} (forall idx$: int :: 
+    (0 <= idx$) && (idx$ < (R[Net#d] + C[Net#d])) ==> (M[Net#d][idx$] == (M[Net#a][idx$] + M[Net#b][idx$]))
+  );
+  assert {:msg "  The network might not preserve the channel invariant"} (forall idx$: int :: 
+    (1 <= idx$) && (idx$ < (R[Net#b] + C[Net#b])) ==> (M[Net#b][idx$] == M[Net#d][idx$ - 1])
+  );
+  assert {:msg "  27.15: The network might not preserve the channel invariant"} (M[Net#b][0] == M[Net#c][-1]) || (M[Net#b][0] == 0);
   C[Net#b] := C[Net#b] - 1;
   assert {:msg "  25.13: The network might not preserve the network invariant"} (M[Net#b][R[Net#b]] == M[Net#c][R[Net#c] - 1]) || (M[Net#b][R[Net#b]] == 0);
   assert {:msg "  19.3: The network might leave unread tokens on channel a"} C[Net#a] == 0;
